thys/Optimized_MTL.thy
@@ -191,7 +191,7 @@ lemma takedropWhile_queue_snd: "snd (takedropWhile_queue f q) = takeWhile f (lin
 
 (* Optimized since data structure *)
 
-type_synonym 'a mmsaux = "ts \<times> ts \<times> \<I> \<times> bool list \<times> bool list \<times>
+type_synonym 'a mmsaux = "ts \<times> ts \<times> bool list \<times> bool list \<times>
   (ts \<times> 'a table) queue \<times> (ts \<times> 'a table) queue \<times>
   (('a tuple, ts) mapping) \<times> (('a tuple, ts) mapping)"
 
@@ -287,21 +287,23 @@ lemma safe_max_Some_dest_in: "finite X \<Longrightarrow> safe_max X = Some x \<L
 lemma safe_max_Some_dest_le: "finite X \<Longrightarrow> safe_max X = Some x \<Longrightarrow> y \<in> X \<Longrightarrow> y \<le> x"
   using Max_ge by (auto simp add: safe_max_def split: if_splits)
 
-fun valid_mmsaux :: "Monitor.window \<Rightarrow> nat \<Rightarrow> nat set \<Rightarrow> nat set \<Rightarrow> 'a mmsaux \<Rightarrow> 'a Monitor.msaux \<Rightarrow>
-  bool" where
-  "valid_mmsaux w n L R (nt, gc, I, maskL, maskR, data_prev, data_in, tuple_in, tuple_since) ys \<longleftrightarrow>
-    L \<subseteq> R \<and> maskL = join_mask n L \<and> maskR = join_mask n R \<and>
-    (\<forall>(t, X) \<in> set ys. table n R X) \<and>
-    table n R (Mapping.keys tuple_in) \<and> table n R (Mapping.keys tuple_since) \<and>
-    (\<forall>as \<in> \<Union>(snd ` (set (linearize data_prev))). wf_tuple n R as) \<and>
-    nt = current w \<and> I = ivl w \<and>
+fun valid_mmsaux :: "args \<Rightarrow> ts \<Rightarrow> 'a mmsaux \<Rightarrow> 'a Monitor.msaux \<Rightarrow> bool" where
+  "valid_mmsaux args cur (nt, gc, maskL, maskR, data_prev, data_in, tuple_in, tuple_since) ys \<longleftrightarrow>
+    (args_L args) \<subseteq> (args_R args) \<and>
+    maskL = join_mask (args_n args) (args_L args) \<and>
+    maskR = join_mask (args_n args) (args_R args) \<and>
+    (\<forall>(t, X) \<in> set ys. table (args_n args) (args_R args) X) \<and>
+    table (args_n args) (args_R args) (Mapping.keys tuple_in) \<and>
+    table (args_n args) (args_R args) (Mapping.keys tuple_since) \<and>
+    (\<forall>as \<in> \<Union>(snd ` (set (linearize data_prev))). wf_tuple (args_n args) (args_R args) as) \<and>
+    cur = nt \<and>
     ts_tuple_rel (set ys) =
     {tas \<in> ts_tuple_rel (set (linearize data_prev) \<union> set (linearize data_in)).
     valid_tuple tuple_since tas} \<and>
     sorted (map fst (linearize data_prev)) \<and>
-    (\<forall>t \<in> fst ` set (linearize data_prev). t \<le> nt \<and> nt - t < left I) \<and>
+    (\<forall>t \<in> fst ` set (linearize data_prev). t \<le> nt \<and> nt - t < left (args_ivl args)) \<and>
     sorted (map fst (linearize data_in)) \<and>
-    (\<forall>t \<in> fst ` set (linearize data_in). t \<le> nt \<and> nt - t \<ge> left I) \<and>
+    (\<forall>t \<in> fst ` set (linearize data_in). t \<le> nt \<and> nt - t \<ge> left (args_ivl args)) \<and>
     (\<forall>as. Mapping.lookup tuple_in as = safe_max (fst `
     {tas \<in> ts_tuple_rel (set (linearize data_in)). valid_tuple tuple_since tas \<and> as = snd tas})) \<and>
     (\<forall>as \<in> Mapping.keys tuple_since. case Mapping.lookup tuple_since as of Some t \<Rightarrow> t \<le> nt)"
@@ -324,19 +326,20 @@ lemma Mapping_keys_dest: "x \<in> Mapping.keys f \<Longrightarrow> \<exists>y. M
 lemma Mapping_keys_intro: "Mapping.lookup f x \<noteq> None \<Longrightarrow> x \<in> Mapping.keys f"
   by (simp add: domIff keys_dom_lookup)
 
-lemma valid_mmsaux_tuple_in_keys: "valid_mmsaux w n L R
-  (nt, gc, I, maskL, maskR, data_prev, data_in, tuple_in, tuple_since) ys \<Longrightarrow>
+lemma valid_mmsaux_tuple_in_keys: "valid_mmsaux args cur
+  (nt, gc, maskL, maskR, data_prev, data_in, tuple_in, tuple_since) ys \<Longrightarrow>
   Mapping.keys tuple_in = snd ` {tas \<in> ts_tuple_rel (set (linearize data_in)).
   valid_tuple tuple_since tas}"
   by (auto intro!: Mapping_keys_intro safe_max_Some_intro
       dest!: Mapping_keys_dest safe_max_Some_dest_in[OF finite_fst_ts_tuple_rel])+
 
-fun init_mmsaux :: "\<I> \<Rightarrow> nat \<Rightarrow> nat set \<Rightarrow> nat set \<Rightarrow> 'a mmsaux" where
-  "init_mmsaux I n L R = (0, 0, I, join_mask n L, join_mask n R,
-  empty_queue, empty_queue, Mapping.empty, Mapping.empty)"
+fun init_mmsaux :: "args \<Rightarrow> 'a mmsaux" where
+  "init_mmsaux args = (0, 0, join_mask (args_n args) (args_L args),
+  join_mask (args_n args) (args_R args), empty_queue, empty_queue, Mapping.empty, Mapping.empty)"
 
-lemma valid_init_mmsaux: "L \<subseteq> R \<Longrightarrow> valid_mmsaux (init_window I) n L R (init_mmsaux I n L R) []"
-  by (auto simp add: init_window_def empty_queue_rep ts_tuple_rel_def join_mask_def
+lemma valid_init_mmsaux: "L \<subseteq> R \<Longrightarrow> valid_mmsaux (init_args I n L R b) 0
+  (init_mmsaux (init_args I n L R b)) []"
+  by (auto simp add: init_args_def empty_queue_rep ts_tuple_rel_def join_mask_def
       Mapping.lookup_empty safe_max_def table_def)
 
 abbreviation "filter_cond X' ts t' \<equiv> (\<lambda>as _. \<not> (as \<in> X' \<and> Mapping.lookup ts as = Some t'))"
@@ -437,24 +440,24 @@ proof (induction ds arbitrary: ts)
   qed
 qed simp
 
-fun filter_mmsaux :: "ts \<Rightarrow> 'a mmsaux \<Rightarrow> 'a mmsaux" where
-  "filter_mmsaux nt (t, gc, I, maskL, maskR, data_prev, data_in, tuple_in, tuple_since) =
-    (let data_prev' = dropWhile_queue (\<lambda>(t, X). enat (nt - t) > right I) data_prev;
+fun shift_end :: "args \<Rightarrow> ts \<Rightarrow> 'a mmsaux \<Rightarrow> 'a mmsaux" where
+  "shift_end args nt (t, gc, maskL, maskR, data_prev, data_in, tuple_in, tuple_since) =
+    (let I = args_ivl args;
+    data_prev' = dropWhile_queue (\<lambda>(t, X). enat (nt - t) > right I) data_prev;
     (data_in, discard) = takedropWhile_queue (\<lambda>(t, X). enat (nt - t) > right I) data_in;
     tuple_in = fold (\<lambda>(t, X) tuple_in. Mapping.filter
       (filter_cond X tuple_in t) tuple_in) discard tuple_in in
-    (t, gc, I, maskL, maskR, data_prev', data_in, tuple_in, tuple_since))"
+    (t, gc, maskL, maskR, data_prev', data_in, tuple_in, tuple_since))"
 
-lemma valid_filter_mmsaux_unfolded:
-  assumes valid_before: "valid_mmsaux w n L R
-    (ot, gc, I, maskL, maskR, data_prev, data_in, tuple_in, tuple_since) auxlist"
-  and nt_mono: "nt \<ge> current w"
-  and new_window: "w' = w\<lparr>earliest := if nt \<ge> right (ivl w)
-    then the_enat (nt - right (ivl w)) else earliest w\<rparr>"
-  shows "valid_mmsaux w' n L R (filter_mmsaux nt
-    (ot, gc, I, maskL, maskR, data_prev, data_in, tuple_in, tuple_since))
-    (filter (\<lambda>(t, rel). enat (nt - t) \<le> right (ivl w)) auxlist)"
+lemma valid_shift_end_mmsaux_unfolded:
+  assumes valid_before: "valid_mmsaux args cur
+    (ot, gc, maskL, maskR, data_prev, data_in, tuple_in, tuple_since) auxlist"
+  and nt_mono: "nt \<ge> cur"
+  shows "valid_mmsaux args cur (shift_end args nt
+    (ot, gc, maskL, maskR, data_prev, data_in, tuple_in, tuple_since))
+    (filter (\<lambda>(t, rel). enat (nt - t) \<le> right (args_ivl args)) auxlist)"
 proof -
+  define I where "I = args_ivl args"
   define data_in' where "data_in' \<equiv>
     fst (takedropWhile_queue (\<lambda>(t, X). enat (nt - t) > right I) data_in)"
   define data_prev' where "data_prev' \<equiv>
@@ -563,7 +566,7 @@ proof -
       qed
     qed
   qed
-  have table_in: "table n R (Mapping.keys tuple_in')"
+  have table_in: "table (args_n args) (args_R args) (Mapping.keys tuple_in')"
     using tuple_in'_keys valid_before by (auto simp add: table_def)
   have "ts_tuple_rel (set auxlist) =
     {as \<in> ts_tuple_rel (set (linearize data_prev) \<union> set (linearize data_in)).
@@ -574,259 +577,17 @@ proof -
     valid_tuple tuple_since as}"
     unfolding lin_data_prev' lin_data_in' ts_tuple_rel_Un ts_tuple_rel_filter by auto
   then show ?thesis
-    using data_prev'_def data_in'_def tuple_in'_def discard_def valid_before nt_mono new_window
+    using data_prev'_def data_in'_def tuple_in'_def discard_def valid_before nt_mono
       sorted_lin_data_prev' sorted_lin_data_in' lin_data_prev' lin_data_in' lookup_tuple_in'
-      table_in
-    by (auto simp only: valid_mmsaux.simps filter_mmsaux.simps Let_def split: prod.splits) auto
+      table_in unfolding I_def
+    by (auto simp only: valid_mmsaux.simps shift_end.simps Let_def split: prod.splits) auto
       (* takes long *)
 qed
 
-lemma valid_filter_mmsaux: "valid_mmsaux w n L R aux auxlist \<Longrightarrow> nt \<ge> current w \<Longrightarrow>
-  w' = w\<lparr>earliest := if nt \<ge> right (ivl w) then the_enat (nt - right (ivl w)) else earliest w\<rparr> \<Longrightarrow>
-  valid_mmsaux w' n L R (filter_mmsaux nt aux)
-  (filter (\<lambda>(t, rel). enat (nt - t) \<le> right (ivl w)) auxlist)"
-  using valid_filter_mmsaux_unfolded by (cases aux) fast
-
-fun join_mmsaux :: "bool \<Rightarrow> 'a table \<Rightarrow> 'a mmsaux \<Rightarrow> 'a mmsaux" where
-  "join_mmsaux pos X (t, gc, I, maskL, maskR, data_prev, data_in, tuple_in, tuple_since) =
-    (if maskL = maskR then
-      (let tuple_in = Mapping.filter (join_filter_cond pos X) tuple_in;
-      tuple_since = Mapping.filter (join_filter_cond pos X) tuple_since in
-      (t, gc, I, maskL, maskR, data_prev, data_in, tuple_in, tuple_since))
-    else if (\<forall>i \<in> set maskL. \<not>i) then
-      (let nones = replicate (length maskL) None;
-      take_all = (pos \<longleftrightarrow> nones \<in> X);
-      tuple_in = (if take_all then tuple_in else Mapping.empty);
-      tuple_since = (if take_all then tuple_since else Mapping.empty) in
-      (t, gc, I, maskL, maskR, data_prev, data_in, tuple_in, tuple_since))
-    else
-      (let tuple_in = Mapping.filter (\<lambda>as _. proj_tuple_in_join pos maskL as X) tuple_in;
-      tuple_since = Mapping.filter (\<lambda>as _. proj_tuple_in_join pos maskL as X) tuple_since in
-      (t, gc, I, maskL, maskR, data_prev, data_in, tuple_in, tuple_since)))"
-
-fun join_mmsaux_abs :: "bool \<Rightarrow> 'a table \<Rightarrow> 'a mmsaux \<Rightarrow> 'a mmsaux" where
-  "join_mmsaux_abs pos X (t, gc, I, maskL, maskR, data_prev, data_in, tuple_in, tuple_since) =
-    (let tuple_in = Mapping.filter (\<lambda>as _. proj_tuple_in_join pos maskL as X) tuple_in;
-    tuple_since = Mapping.filter (\<lambda>as _. proj_tuple_in_join pos maskL as X) tuple_since in
-    (t, gc, I, maskL, maskR, data_prev, data_in, tuple_in, tuple_since))"
-
-lemma Mapping_filter_cong:
-  assumes cong: "(\<And>k v. k \<in> Mapping.keys m \<Longrightarrow> f k v = f' k v)"
-  shows "Mapping.filter f m = Mapping.filter f' m"
-proof -
-  have "\<And>k. Mapping.lookup (Mapping.filter f m) k = Mapping.lookup (Mapping.filter f' m) k"
-    using cong
-    by (fastforce simp add: Mapping.lookup_filter intro: Mapping_keys_intro split: option.splits)
-  then show ?thesis
-    by (simp add: mapping_eqI)
-qed
-
-lemma join_mmsaux_abs_eq:
-  assumes valid_before: "valid_mmsaux w n L R
-    (nt, gc, I, maskL, maskR, data_prev, data_in, tuple_in, tuple_since) auxlist"
-  and table_left: "table n L X"
-  shows "join_mmsaux pos X (nt, gc, I, maskL, maskR, data_prev, data_in, tuple_in, tuple_since) =
-    join_mmsaux_abs pos X (nt, gc, I, maskL, maskR, data_prev, data_in, tuple_in, tuple_since)"
-proof (cases "maskL = maskR")
-  case True
-  have keys_wf_in: "\<And>as. as \<in> Mapping.keys tuple_in \<Longrightarrow> wf_tuple n L as"
-    using wf_tuple_change_base valid_before True by (fastforce simp add: table_def)
-  have cong_in: "\<And>as n. as \<in> Mapping.keys tuple_in \<Longrightarrow>
-    proj_tuple_in_join pos maskL as X \<longleftrightarrow> join_cond pos X as"
-    using proj_tuple_in_join_mask_idle[OF keys_wf_in] valid_before
-    by (auto simp only: valid_mmsaux.simps)
-  have keys_wf_since: "\<And>as. as \<in> Mapping.keys tuple_since \<Longrightarrow> wf_tuple n L as"
-    using wf_tuple_change_base valid_before True by (fastforce simp add: table_def)
-  have cong_since: "\<And>as n. as \<in> Mapping.keys tuple_since \<Longrightarrow>
-    proj_tuple_in_join pos maskL as X \<longleftrightarrow> join_cond pos X as"
-    using proj_tuple_in_join_mask_idle[OF keys_wf_since] valid_before
-    by (auto simp only: valid_mmsaux.simps)
-  show ?thesis
-    using True Mapping_filter_cong[OF cong_in, of tuple_in "\<lambda>k _. k"]
-      Mapping_filter_cong[OF cong_since, of tuple_since "\<lambda>k _. k"]
-    by auto
-next
-  case False
-  then show ?thesis
-  proof (cases "\<forall>i \<in> set maskL. \<not>i")
-    case True
-    have length_maskL: "length maskL = n"
-      using valid_before by (auto simp add: join_mask_def)
-    have proj_rep: "\<And>as. wf_tuple n R as \<Longrightarrow> proj_tuple maskL as = replicate (length maskL) None"
-      using True proj_tuple_replicate by (force simp add: length_maskL wf_tuple_def)
-    have keys_wf_in: "\<And>as. as \<in> Mapping.keys tuple_in \<Longrightarrow> wf_tuple n R as"
-      using valid_before by (auto simp add: table_def)
-    have keys_wf_since: "\<And>as. as \<in> Mapping.keys tuple_since \<Longrightarrow> wf_tuple n R as"
-      using valid_before by (auto simp add: table_def)
-    have "\<And>as. Mapping.lookup (Mapping.filter (\<lambda>as _. proj_tuple_in_join pos maskL as X)
-      tuple_in) as = Mapping.lookup (if (pos \<longleftrightarrow> replicate (length maskL) None \<in> X)
-      then tuple_in else Mapping.empty) as"
-      using proj_rep[OF keys_wf_in]
-      by (auto simp add: Mapping.lookup_filter Mapping.lookup_empty proj_tuple_in_join_def
-          Mapping_keys_intro split: option.splits)
-    moreover have "\<And>as. Mapping.lookup (Mapping.filter (\<lambda>as _. proj_tuple_in_join pos maskL as X)
-      tuple_since) as = Mapping.lookup (if (pos \<longleftrightarrow> replicate (length maskL) None \<in> X)
-      then tuple_since else Mapping.empty) as"
-      using proj_rep[OF keys_wf_since]
-      by (auto simp add: Mapping.lookup_filter Mapping.lookup_empty proj_tuple_in_join_def
-          Mapping_keys_intro split: option.splits)
-    ultimately show ?thesis
-      using False True by (auto simp add: mapping_eqI Let_def)
-  qed auto
-qed
-
-lemma valid_join_mmsaux_unfolded:
-  assumes valid_before: "valid_mmsaux w n L R
-    (nt, gc, I, maskL, maskR, data_prev, data_in, tuple_in, tuple_since) auxlist"
-  and table_left: "table n L X"
-  shows "valid_mmsaux w n L R
-    (join_mmsaux pos X (nt, gc, I, maskL, maskR, data_prev, data_in, tuple_in, tuple_since))
-    (map (\<lambda>(t, rel). (t, join rel pos X)) auxlist)"
-proof -
-  define tuple_in' where "tuple_in' \<equiv>
-    Mapping.filter (\<lambda>as _. proj_tuple_in_join pos maskL as X) tuple_in"
-  define tuple_since' where "tuple_since' \<equiv>
-    Mapping.filter (\<lambda>as _. proj_tuple_in_join pos maskL as X) tuple_since"
-  have tuple_in_None_None: "\<And>as. Mapping.lookup tuple_in as = None \<Longrightarrow>
-    Mapping.lookup tuple_in' as = None"
-    unfolding tuple_in'_def using Mapping_lookup_filter_not_None by fastforce
-  have tuple_in'_keys: "\<And>as. as \<in> Mapping.keys tuple_in' \<Longrightarrow> as \<in> Mapping.keys tuple_in"
-    using tuple_in_None_None
-    by (fastforce intro: Mapping_keys_intro dest: Mapping_keys_dest)
-  have tuple_since_None_None: "\<And>as. Mapping.lookup tuple_since as = None \<Longrightarrow>
-    Mapping.lookup tuple_since' as = None"
-    unfolding tuple_since'_def using Mapping_lookup_filter_not_None by fastforce
-  have tuple_since'_keys: "\<And>as. as \<in> Mapping.keys tuple_since' \<Longrightarrow> as \<in> Mapping.keys tuple_since"
-    using tuple_since_None_None
-    by (fastforce intro: Mapping_keys_intro dest: Mapping_keys_dest)
-  have ts_tuple_rel': "ts_tuple_rel (set (map (\<lambda>(t, rel). (t, join rel pos X)) auxlist)) =
-    {tas \<in> ts_tuple_rel (set (linearize data_prev) \<union> set (linearize data_in)).
-    valid_tuple tuple_since' tas}"
-  proof (rule set_eqI, rule iffI)
-    fix tas
-    assume assm: "tas \<in> ts_tuple_rel (set (map (\<lambda>(t, rel). (t, join rel pos X)) auxlist))"
-    then obtain t as Z where tas_def: "tas = (t, as)" "as \<in> join Z pos X" "(t, Z) \<in> set auxlist"
-      "(t, join Z pos X) \<in> set (map (\<lambda>(t, rel). (t, join rel pos X)) auxlist)"
-      by (fastforce simp add: ts_tuple_rel_def)
-    from tas_def(3) have table_Z: "table n R Z"
-      using valid_before by auto
-    have proj: "as \<in> Z" "proj_tuple_in_join pos maskL as X"
-      using tas_def(2) join_sub[OF _ table_left table_Z] valid_before by auto
-    then have "(t, as) \<in> ts_tuple_rel (set (auxlist))"
-      using tas_def(3) by (auto simp add: ts_tuple_rel_def)
-    then have tas_in: "(t, as) \<in> ts_tuple_rel
-      (set (linearize data_prev) \<union> set (linearize data_in))" "valid_tuple tuple_since (t, as)"
-      using valid_before by auto
-    then obtain t' where t'_def: "Mapping.lookup tuple_since as = Some t'" "t \<ge> t'"
-      by (auto simp add: valid_tuple_def split: option.splits)
-    then have valid_tuple_since': "valid_tuple tuple_since' (t, as)"
-      using proj(2)
-      by (auto simp add: tuple_since'_def Mapping_lookup_filter_Some valid_tuple_def)
-    show "tas \<in> {tas \<in> ts_tuple_rel (set (linearize data_prev) \<union> set (linearize data_in)).
-      valid_tuple tuple_since' tas}"
-      using tas_in valid_tuple_since' unfolding tas_def(1)[symmetric] by auto
-  next
-    fix tas
-    assume assm: "tas \<in> {tas \<in> ts_tuple_rel
-      (set (linearize data_prev) \<union> set (linearize data_in)). valid_tuple tuple_since' tas}"
-    then obtain t as where tas_def: "tas = (t, as)" "valid_tuple tuple_since' (t, as)"
-      by (auto simp add: ts_tuple_rel_def)
-    from tas_def(2) have "valid_tuple tuple_since (t, as)"
-      unfolding tuple_since'_def using Mapping_lookup_filter_not_None
-      by (force simp add: valid_tuple_def split: option.splits)
-    then have "(t, as) \<in> ts_tuple_rel (set auxlist)"
-      using valid_before assm tas_def(1) by auto
-    then obtain Z where Z_def: "as \<in> Z" "(t, Z) \<in> set auxlist"
-      by (auto simp add: ts_tuple_rel_def)
-    then have table_Z: "table n R Z"
-      using valid_before by auto
-    from tas_def(2) have "proj_tuple_in_join pos maskL as X"
-      unfolding tuple_since'_def using Mapping_lookup_filter_Some_P
-      by (fastforce simp add: valid_tuple_def split: option.splits)
-    then have as_in_join: "as \<in> join Z pos X"
-      using join_sub[OF _ table_left table_Z] Z_def(1) valid_before by auto
-    then show "tas \<in> ts_tuple_rel (set (map (\<lambda>(t, rel). (t, join rel pos X)) auxlist))"
-      using Z_def unfolding tas_def(1) by (auto simp add: ts_tuple_rel_def)
-  qed
-  have lookup_tuple_in': "\<And>as. Mapping.lookup tuple_in' as = safe_max (fst `
-    {tas \<in> ts_tuple_rel (set (linearize data_in)). valid_tuple tuple_since' tas \<and> as = snd tas})"
-  proof -
-    fix as
-    show "Mapping.lookup tuple_in' as = safe_max (fst `
-    {tas \<in> ts_tuple_rel (set (linearize data_in)). valid_tuple tuple_since' tas \<and> as = snd tas})"
-    proof (cases "Mapping.lookup tuple_in as")
-      case None
-      then have "{tas \<in> ts_tuple_rel (set (linearize data_in)).
-        valid_tuple tuple_since tas \<and> as = snd tas} = {}"
-        using valid_before by (auto dest!: safe_max_empty_dest)
-      then have "{tas \<in> ts_tuple_rel (set (linearize data_in)).
-        valid_tuple tuple_since' tas \<and> as = snd tas} = {}"
-        using Mapping_lookup_filter_not_None
-        by (fastforce simp add: valid_tuple_def tuple_since'_def split: option.splits)
-      then show ?thesis
-        unfolding tuple_in_None_None[OF None] using iffD2[OF safe_max_empty, symmetric] by blast
-    next
-      case (Some t)
-      show ?thesis
-      proof (cases "proj_tuple_in_join pos maskL as X")
-        case True
-        then have lookup_tuple_in': "Mapping.lookup tuple_in' as = Some t"
-          using Some unfolding tuple_in'_def by (simp add: Mapping_lookup_filter_Some)
-        have "(t, as) \<in> ts_tuple_rel (set (linearize data_in))" "valid_tuple tuple_since (t, as)"
-          using valid_before Some by (auto dest: safe_max_Some_dest_in[OF finite_fst_ts_tuple_rel])
-        then have t_in_fst: "t \<in> fst ` {tas \<in> ts_tuple_rel (set (linearize data_in)).
-          valid_tuple tuple_since' tas \<and> as = snd tas}"
-          using True by (auto simp add: image_iff valid_tuple_def tuple_since'_def
-            Mapping_lookup_filter_Some split: option.splits)
-        have "\<And>t'. valid_tuple tuple_since' (t', as) \<Longrightarrow> valid_tuple tuple_since (t', as)"
-          using Mapping_lookup_filter_not_None
-          by (fastforce simp add: valid_tuple_def tuple_since'_def split: option.splits)
-        then have "\<And>t'. (t', as) \<in> ts_tuple_rel (set (linearize data_in)) \<Longrightarrow>
-          valid_tuple tuple_since' (t', as) \<Longrightarrow> t' \<le> t"
-          using valid_before Some safe_max_Some_dest_le[OF finite_fst_ts_tuple_rel]
-          by (fastforce simp add: image_iff)
-        then have "Max (fst ` {tas \<in> ts_tuple_rel (set (linearize data_in)).
-          valid_tuple tuple_since' tas \<and> as = snd tas}) = t"
-          using Max_eqI[OF finite_fst_ts_tuple_rel[of "linearize data_in"],
-            OF _ t_in_fst] by fastforce
-        then show ?thesis
-          unfolding lookup_tuple_in' using t_in_fst by (auto simp add: safe_max_def)
-      next
-        case False
-        then have lookup_tuple': "Mapping.lookup tuple_in' as = None"
-          "Mapping.lookup tuple_since' as = None"
-          unfolding tuple_in'_def tuple_since'_def
-          by (auto simp add: Mapping_lookup_filter_None)
-        then have "\<And>tas. \<not>(valid_tuple tuple_since' tas \<and> as = snd tas)"
-          by (auto simp add: valid_tuple_def split: option.splits)
-        then show ?thesis
-          unfolding lookup_tuple' by (auto simp add: safe_max_def)
-      qed
-    qed
-  qed
-  have table_join': "\<And>t ys. (t, ys) \<in> set auxlist \<Longrightarrow> table n R (join ys pos X)"
-  proof -
-    fix t ys
-    assume "(t, ys) \<in> set auxlist"
-    then have table_ys: "table n R ys"
-      using valid_before by auto
-    show "table n R (join ys pos X)"
-      using join_table[OF table_ys table_left, of pos R] valid_before by auto
-  qed
-  have table_in': "table n R (Mapping.keys tuple_in')"
-    using tuple_in'_keys valid_before by (auto simp add: table_def)
-  have table_since': "table n R (Mapping.keys tuple_since')"
-    using tuple_since'_keys valid_before by (auto simp add: table_def)
-  show ?thesis
-    unfolding join_mmsaux_abs_eq[OF valid_before table_left]
-    using valid_before ts_tuple_rel' lookup_tuple_in' tuple_in'_def tuple_since'_def table_join'
-      Mapping_filter_keys[of tuple_since "\<lambda>as. case as of Some t \<Rightarrow> t \<le> nt"]
-      table_in' table_since' by auto
-qed
-
-lemma valid_join_mmsaux: "valid_mmsaux w n L R aux auxlist \<Longrightarrow> table n L X \<Longrightarrow>
-  valid_mmsaux w n L R (join_mmsaux pos X aux) (map (\<lambda>(t, rel). (t, join rel pos X)) auxlist)"
-  using valid_join_mmsaux_unfolded by (cases aux) fast
+lemma valid_shift_end_mmsaux: "valid_mmsaux args cur aux auxlist \<Longrightarrow> nt \<ge> cur \<Longrightarrow>
+  valid_mmsaux args cur (shift_end args nt aux)
+  (filter (\<lambda>(t, rel). enat (nt - t) \<le> right (args_ivl args)) auxlist)"
+  using valid_shift_end_mmsaux_unfolded by (cases aux) fast
 
 setup_lifting type_definition_mapping
 
@@ -915,27 +676,31 @@ proof (induction xs arbitrary: m)
   qed
 qed simp
 
-fun add_new_ts_mmsaux :: "ts \<Rightarrow> 'a mmsaux \<Rightarrow> 'a mmsaux" where
-  "add_new_ts_mmsaux nt (t, gc, I, maskL, maskR, data_prev, data_in, tuple_in, tuple_since) =
-    (let (data_prev, move) = takedropWhile_queue (\<lambda>(t, X). nt - t \<ge> left I) data_prev;
+fun add_new_ts_mmsaux' :: "args \<Rightarrow> ts \<Rightarrow> 'a mmsaux \<Rightarrow> 'a mmsaux" where
+  "add_new_ts_mmsaux' args nt (t, gc, maskL, maskR, data_prev, data_in, tuple_in, tuple_since) =
+    (let I = args_ivl args;
+    (data_prev, move) = takedropWhile_queue (\<lambda>(t, X). nt - t \<ge> left I) data_prev;
     data_in = fold (\<lambda>(t, X) data_in. append_queue (t, X) data_in) move data_in;
     tuple_in = fold (\<lambda>(t, X) tuple_in. upd_set tuple_in (\<lambda>_. t)
       {as \<in> X. valid_tuple tuple_since (t, as)}) move tuple_in in
-    (nt, gc, I, maskL, maskR, data_prev, data_in, tuple_in, tuple_since))"
+    (nt, gc, maskL, maskR, data_prev, data_in, tuple_in, tuple_since))"
 
 lemma Mapping_keys_fold_upd_set: "k \<in> Mapping.keys (fold (\<lambda>(t, X) m. upd_set m (\<lambda>_. t) (Z t X))
   xs m) \<Longrightarrow> k \<in> Mapping.keys m \<or> (\<exists>(t, X) \<in> set xs. k \<in> Z t X)"
   by (induction xs arbitrary: m) (fastforce simp add: Mapping_upd_set_keys)+
 
-lemma valid_add_new_ts_mmsaux_unfolded:
-  assumes valid_before: "valid_mmsaux w n L R
-    (ot, gc, I, maskL, maskR, data_prev, data_in, tuple_in, tuple_since) auxlist"
-  and nt_mono: "nt \<ge> current w"
-  and new_window: "w' = w\<lparr>latest := if nt \<ge> left (ivl w)
-    then nt - left (ivl w) else latest w, current := nt\<rparr>"
-  shows "valid_mmsaux w' n L R (add_new_ts_mmsaux nt
-    (ot, gc, I, maskL, maskR, data_prev, data_in, tuple_in, tuple_since)) auxlist"
+lemma valid_add_new_ts_mmsaux'_unfolded:
+  assumes valid_before: "valid_mmsaux args cur
+    (ot, gc, maskL, maskR, data_prev, data_in, tuple_in, tuple_since) auxlist"
+  and nt_mono: "nt \<ge> cur"
+  shows "valid_mmsaux args nt (add_new_ts_mmsaux' args nt
+    (ot, gc, maskL, maskR, data_prev, data_in, tuple_in, tuple_since)) auxlist"
 proof -
+  define I where "I = args_ivl args"
+  define n where "n = args_n args"
+  define L where "L = args_L args"
+  define R where "R = args_R args"
+  define pos where "pos = args_pos args"
   define data_prev' where "data_prev' \<equiv> dropWhile_queue (\<lambda>(t, X). nt - t \<ge> left I) data_prev"
   define move where "move \<equiv> takeWhile (\<lambda>(t, X). nt - t \<ge> left I) (linearize data_prev)"
   define data_in' where "data_in' \<equiv> fold (\<lambda>(t, X) data_in. append_queue (t, X) data_in)
@@ -948,10 +713,10 @@ proof -
     by (auto simp add: tuple_in'_def)
   have F1: "sorted (map fst (linearize data_in))" "\<forall>t \<in> fst ` set (linearize data_in). t \<le> nt"
     "\<forall>t \<in> fst ` set (linearize data_in). t \<le> ot \<and> ot - t \<ge> left I"
-    using valid_before nt_mono by auto
+    using valid_before nt_mono unfolding I_def by auto
   have F2: "sorted (map fst (linearize data_prev))" "\<forall>t \<in> fst ` set (linearize data_prev). t \<le> nt"
     "\<forall>t \<in> fst ` set (linearize data_prev). t \<le> ot \<and> ot - t < left I"
-    using valid_before nt_mono by auto
+    using valid_before nt_mono unfolding I_def by auto
   have lin_data_prev': "linearize data_prev' =
     filter (\<lambda>(t, X). nt - t < left I) (linearize data_prev)"
     unfolding data_prev'_def dropWhile_queue_rep dropWhile_filter'[OF F2(1,2)] ..
@@ -1044,7 +809,7 @@ proof -
       proof (rule disjE)
         assume "as \<in> Mapping.keys tuple_in"
         then show "wf_tuple n R as"
-          using valid_before by (auto simp add: table_def)
+          using valid_before by (auto simp add: table_def n_def R_def)
       next
         assume "\<exists>(t, X)\<in>set move. as \<in> {as \<in> X. valid_tuple tuple_since (t, as)}"
         then obtain t X where tX_def: "(t, X) \<in> set move" "as \<in> X"
@@ -1052,7 +817,7 @@ proof -
         then have "as \<in> \<Union>(snd ` set (linearize data_prev))"
           unfolding move_def using set_takeWhileD by force
         then show "wf_tuple n R as"
-          using valid_before by auto
+          using valid_before by (auto simp add: n_def R_def)
       qed
     }
     then show ?thesis
@@ -1062,39 +827,401 @@ proof -
     takedropWhile_queue (\<lambda>(t, X). nt - t \<ge> left I) data_prev"
     using takedropWhile_queue_fst takedropWhile_queue_snd data_prev'_def move_def
     by (metis surjective_pairing)
-  moreover have "valid_mmsaux w' n L R (nt, gc, I, maskL, maskR, data_prev', data_in',
+  moreover have "valid_mmsaux args nt (nt, gc, maskL, maskR, data_prev', data_in',
     tuple_in', tuple_since) auxlist"
     using lin_data_prev' sorted_lin_data_prev' lin_data_in' move_filter sorted_lin_data_in'
-      nt_mono valid_before ts_tuple_rel' lookup' new_window table_in'
-    by (auto simp only: valid_mmsaux.simps split: option.splits) auto
+      nt_mono valid_before ts_tuple_rel' lookup' table_in' unfolding I_def
+    by (auto simp only: valid_mmsaux.simps Let_def n_def R_def split: option.splits) auto
       (* takes long *)
   ultimately show ?thesis
-    by (auto simp only: add_new_ts_mmsaux.simps Let_def data_in'_def tuple_in'_def
+    by (auto simp only: add_new_ts_mmsaux'.simps Let_def data_in'_def tuple_in'_def I_def
         split: prod.splits)
 qed
 
-lemma valid_add_new_ts_mmsaux: "valid_mmsaux w n L R aux auxlist \<Longrightarrow> nt \<ge> current w \<Longrightarrow>
-  w' = w\<lparr>latest := if nt \<ge> left (ivl w) then nt - left (ivl w) else latest w, current := nt\<rparr> \<Longrightarrow>
-  valid_mmsaux w' n L R (add_new_ts_mmsaux nt aux) auxlist"
-  using valid_add_new_ts_mmsaux_unfolded by (cases aux) fast
+lemma valid_add_new_ts_mmsaux': "valid_mmsaux args cur aux auxlist \<Longrightarrow> nt \<ge> cur \<Longrightarrow>
+  valid_mmsaux args nt (add_new_ts_mmsaux' args nt aux) auxlist"
+  using valid_add_new_ts_mmsaux'_unfolded by (cases aux) fast
 
-fun add_new_table_mmsaux :: "'a table \<Rightarrow> 'a mmsaux \<Rightarrow> 'a mmsaux" where
-  "add_new_table_mmsaux X (t, gc, I, maskL, maskR, data_prev, data_in, tuple_in, tuple_since) =
+definition add_new_ts_mmsaux :: "args \<Rightarrow> ts \<Rightarrow> 'a mmsaux \<Rightarrow> 'a mmsaux" where
+  "add_new_ts_mmsaux args nt aux = add_new_ts_mmsaux' args nt (shift_end args nt aux)"
+
+lemma valid_add_new_ts_mmsaux:
+  assumes "valid_mmsaux args cur aux auxlist" "nt \<ge> cur"
+  shows "valid_mmsaux args nt (add_new_ts_mmsaux args nt aux)
+    (filter (\<lambda>(t, rel). enat (nt - t) \<le> right (args_ivl args)) auxlist)"
+  using valid_add_new_ts_mmsaux'[OF valid_shift_end_mmsaux[OF assms] assms(2)]
+  unfolding add_new_ts_mmsaux_def .
+
+fun join_mmsaux :: "args \<Rightarrow> 'a table \<Rightarrow> 'a mmsaux \<Rightarrow> 'a mmsaux" where
+  "join_mmsaux args X (t, gc, maskL, maskR, data_prev, data_in, tuple_in, tuple_since) =
+    (let pos = args_pos args in
+    (if maskL = maskR then
+      (let tuple_in = Mapping.filter (join_filter_cond pos X) tuple_in;
+      tuple_since = Mapping.filter (join_filter_cond pos X) tuple_since in
+      (t, gc, maskL, maskR, data_prev, data_in, tuple_in, tuple_since))
+    else if (\<forall>i \<in> set maskL. \<not>i) then
+      (let nones = replicate (length maskL) None;
+      take_all = (pos \<longleftrightarrow> nones \<in> X);
+      tuple_in = (if take_all then tuple_in else Mapping.empty);
+      tuple_since = (if take_all then tuple_since else Mapping.empty) in
+      (t, gc, maskL, maskR, data_prev, data_in, tuple_in, tuple_since))
+    else
+      (let tuple_in = Mapping.filter (\<lambda>as _. proj_tuple_in_join pos maskL as X) tuple_in;
+      tuple_since = Mapping.filter (\<lambda>as _. proj_tuple_in_join pos maskL as X) tuple_since in
+      (t, gc, maskL, maskR, data_prev, data_in, tuple_in, tuple_since))))"
+
+fun join_mmsaux_abs :: "args \<Rightarrow> 'a table \<Rightarrow> 'a mmsaux \<Rightarrow> 'a mmsaux" where
+  "join_mmsaux_abs args X (t, gc, maskL, maskR, data_prev, data_in, tuple_in, tuple_since) =
+    (let pos = args_pos args in
+    (let tuple_in = Mapping.filter (\<lambda>as _. proj_tuple_in_join pos maskL as X) tuple_in;
+    tuple_since = Mapping.filter (\<lambda>as _. proj_tuple_in_join pos maskL as X) tuple_since in
+    (t, gc, maskL, maskR, data_prev, data_in, tuple_in, tuple_since)))"
+
+lemma Mapping_filter_cong:
+  assumes cong: "(\<And>k v. k \<in> Mapping.keys m \<Longrightarrow> f k v = f' k v)"
+  shows "Mapping.filter f m = Mapping.filter f' m"
+proof -
+  have "\<And>k. Mapping.lookup (Mapping.filter f m) k = Mapping.lookup (Mapping.filter f' m) k"
+    using cong
+    by (fastforce simp add: Mapping.lookup_filter intro: Mapping_keys_intro split: option.splits)
+  then show ?thesis
+    by (simp add: mapping_eqI)
+qed
+
+lemma join_mmsaux_abs_eq:
+  assumes valid_before: "valid_mmsaux args cur
+    (nt, gc, maskL, maskR, data_prev, data_in, tuple_in, tuple_since) auxlist"
+  and table_left: "table (args_n args) (args_L args) X"
+  shows "join_mmsaux args X (nt, gc, maskL, maskR, data_prev, data_in, tuple_in, tuple_since) =
+    join_mmsaux_abs args X (nt, gc, maskL, maskR, data_prev, data_in, tuple_in, tuple_since)"
+proof (cases "maskL = maskR")
+  case True
+  define n where "n = args_n args"
+  define L where "L = args_L args"
+  define pos where "pos = args_pos args"
+  have keys_wf_in: "\<And>as. as \<in> Mapping.keys tuple_in \<Longrightarrow> wf_tuple n L as"
+    using wf_tuple_change_base valid_before True by (fastforce simp add: table_def n_def L_def)
+  have cong_in: "\<And>as n. as \<in> Mapping.keys tuple_in \<Longrightarrow>
+    proj_tuple_in_join pos maskL as X \<longleftrightarrow> join_cond pos X as"
+    using proj_tuple_in_join_mask_idle[OF keys_wf_in] valid_before
+    by (auto simp only: valid_mmsaux.simps n_def L_def pos_def)
+  have keys_wf_since: "\<And>as. as \<in> Mapping.keys tuple_since \<Longrightarrow> wf_tuple n L as"
+    using wf_tuple_change_base valid_before True by (fastforce simp add: table_def n_def L_def)
+  have cong_since: "\<And>as n. as \<in> Mapping.keys tuple_since \<Longrightarrow>
+    proj_tuple_in_join pos maskL as X \<longleftrightarrow> join_cond pos X as"
+    using proj_tuple_in_join_mask_idle[OF keys_wf_since] valid_before
+    by (auto simp only: valid_mmsaux.simps n_def L_def pos_def)
+  show ?thesis
+    using True Mapping_filter_cong[OF cong_in, of tuple_in "\<lambda>k _. k"]
+      Mapping_filter_cong[OF cong_since, of tuple_since "\<lambda>k _. k"]
+    by (auto simp add: pos_def)
+next
+  case False
+  define n where "n = args_n args"
+  define L where "L = args_L args"
+  define R where "R = args_R args"
+  define pos where "pos = args_pos args"
+  from False show ?thesis
+  proof (cases "\<forall>i \<in> set maskL. \<not>i")
+    case True
+    have length_maskL: "length maskL = n"
+      using valid_before by (auto simp add: join_mask_def n_def)
+    have proj_rep: "\<And>as. wf_tuple n R as \<Longrightarrow> proj_tuple maskL as = replicate (length maskL) None"
+      using True proj_tuple_replicate by (force simp add: length_maskL wf_tuple_def)
+    have keys_wf_in: "\<And>as. as \<in> Mapping.keys tuple_in \<Longrightarrow> wf_tuple n R as"
+      using valid_before by (auto simp add: table_def n_def R_def)
+    have keys_wf_since: "\<And>as. as \<in> Mapping.keys tuple_since \<Longrightarrow> wf_tuple n R as"
+      using valid_before by (auto simp add: table_def n_def R_def)
+    have "\<And>as. Mapping.lookup (Mapping.filter (\<lambda>as _. proj_tuple_in_join pos maskL as X)
+      tuple_in) as = Mapping.lookup (if (pos \<longleftrightarrow> replicate (length maskL) None \<in> X)
+      then tuple_in else Mapping.empty) as"
+      using proj_rep[OF keys_wf_in]
+      by (auto simp add: Mapping.lookup_filter Mapping.lookup_empty proj_tuple_in_join_def
+          Mapping_keys_intro split: option.splits)
+    moreover have "\<And>as. Mapping.lookup (Mapping.filter (\<lambda>as _. proj_tuple_in_join pos maskL as X)
+      tuple_since) as = Mapping.lookup (if (pos \<longleftrightarrow> replicate (length maskL) None \<in> X)
+      then tuple_since else Mapping.empty) as"
+      using proj_rep[OF keys_wf_since]
+      by (auto simp add: Mapping.lookup_filter Mapping.lookup_empty proj_tuple_in_join_def
+          Mapping_keys_intro split: option.splits)
+    ultimately show ?thesis
+      using False True by (auto simp add: mapping_eqI Let_def pos_def)
+  qed (auto simp add: Let_def)
+qed
+
+lemma valid_join_mmsaux_unfolded:
+  assumes valid_before: "valid_mmsaux args cur
+    (nt, gc, maskL, maskR, data_prev, data_in, tuple_in, tuple_since) auxlist"
+  and table_left': "table (args_n args) (args_L args) X"
+  shows "valid_mmsaux args cur
+    (join_mmsaux args X (nt, gc, maskL, maskR, data_prev, data_in, tuple_in, tuple_since))
+    (map (\<lambda>(t, rel). (t, join rel (args_pos args) X)) auxlist)"
+proof -
+  define n where "n = args_n args"
+  define L where "L = args_L args"
+  define R where "R = args_R args"
+  define pos where "pos = args_pos args"
+  note table_left = table_left'[unfolded n_def[symmetric] L_def[symmetric]]
+  define tuple_in' where "tuple_in' \<equiv>
+    Mapping.filter (\<lambda>as _. proj_tuple_in_join pos maskL as X) tuple_in"
+  define tuple_since' where "tuple_since' \<equiv>
+    Mapping.filter (\<lambda>as _. proj_tuple_in_join pos maskL as X) tuple_since"
+  have tuple_in_None_None: "\<And>as. Mapping.lookup tuple_in as = None \<Longrightarrow>
+    Mapping.lookup tuple_in' as = None"
+    unfolding tuple_in'_def using Mapping_lookup_filter_not_None by fastforce
+  have tuple_in'_keys: "\<And>as. as \<in> Mapping.keys tuple_in' \<Longrightarrow> as \<in> Mapping.keys tuple_in"
+    using tuple_in_None_None
+    by (fastforce intro: Mapping_keys_intro dest: Mapping_keys_dest)
+  have tuple_since_None_None: "\<And>as. Mapping.lookup tuple_since as = None \<Longrightarrow>
+    Mapping.lookup tuple_since' as = None"
+    unfolding tuple_since'_def using Mapping_lookup_filter_not_None by fastforce
+  have tuple_since'_keys: "\<And>as. as \<in> Mapping.keys tuple_since' \<Longrightarrow> as \<in> Mapping.keys tuple_since"
+    using tuple_since_None_None
+    by (fastforce intro: Mapping_keys_intro dest: Mapping_keys_dest)
+  have ts_tuple_rel': "ts_tuple_rel (set (map (\<lambda>(t, rel). (t, join rel pos X)) auxlist)) =
+    {tas \<in> ts_tuple_rel (set (linearize data_prev) \<union> set (linearize data_in)).
+    valid_tuple tuple_since' tas}"
+  proof (rule set_eqI, rule iffI)
+    fix tas
+    assume assm: "tas \<in> ts_tuple_rel (set (map (\<lambda>(t, rel). (t, join rel pos X)) auxlist))"
+    then obtain t as Z where tas_def: "tas = (t, as)" "as \<in> join Z pos X" "(t, Z) \<in> set auxlist"
+      "(t, join Z pos X) \<in> set (map (\<lambda>(t, rel). (t, join rel pos X)) auxlist)"
+      by (fastforce simp add: ts_tuple_rel_def)
+    from tas_def(3) have table_Z: "table n R Z"
+      using valid_before by (auto simp add: n_def R_def)
+    have proj: "as \<in> Z" "proj_tuple_in_join pos maskL as X"
+      using tas_def(2) join_sub[OF _ table_left table_Z] valid_before
+      by (auto simp add: n_def L_def R_def pos_def)
+    then have "(t, as) \<in> ts_tuple_rel (set (auxlist))"
+      using tas_def(3) by (auto simp add: ts_tuple_rel_def)
+    then have tas_in: "(t, as) \<in> ts_tuple_rel
+      (set (linearize data_prev) \<union> set (linearize data_in))" "valid_tuple tuple_since (t, as)"
+      using valid_before by auto
+    then obtain t' where t'_def: "Mapping.lookup tuple_since as = Some t'" "t \<ge> t'"
+      by (auto simp add: valid_tuple_def split: option.splits)
+    then have valid_tuple_since': "valid_tuple tuple_since' (t, as)"
+      using proj(2)
+      by (auto simp add: tuple_since'_def Mapping_lookup_filter_Some valid_tuple_def)
+    show "tas \<in> {tas \<in> ts_tuple_rel (set (linearize data_prev) \<union> set (linearize data_in)).
+      valid_tuple tuple_since' tas}"
+      using tas_in valid_tuple_since' unfolding tas_def(1)[symmetric] by auto
+  next
+    fix tas
+    assume assm: "tas \<in> {tas \<in> ts_tuple_rel
+      (set (linearize data_prev) \<union> set (linearize data_in)). valid_tuple tuple_since' tas}"
+    then obtain t as where tas_def: "tas = (t, as)" "valid_tuple tuple_since' (t, as)"
+      by (auto simp add: ts_tuple_rel_def)
+    from tas_def(2) have "valid_tuple tuple_since (t, as)"
+      unfolding tuple_since'_def using Mapping_lookup_filter_not_None
+      by (force simp add: valid_tuple_def split: option.splits)
+    then have "(t, as) \<in> ts_tuple_rel (set auxlist)"
+      using valid_before assm tas_def(1) by auto
+    then obtain Z where Z_def: "as \<in> Z" "(t, Z) \<in> set auxlist"
+      by (auto simp add: ts_tuple_rel_def)
+    then have table_Z: "table n R Z"
+      using valid_before by (auto simp add: n_def R_def)
+    from tas_def(2) have "proj_tuple_in_join pos maskL as X"
+      unfolding tuple_since'_def using Mapping_lookup_filter_Some_P
+      by (fastforce simp add: valid_tuple_def split: option.splits)
+    then have as_in_join: "as \<in> join Z pos X"
+      using join_sub[OF _ table_left table_Z] Z_def(1) valid_before
+      by (auto simp add: n_def L_def R_def pos_def)
+    then show "tas \<in> ts_tuple_rel (set (map (\<lambda>(t, rel). (t, join rel pos X)) auxlist))"
+      using Z_def unfolding tas_def(1) by (auto simp add: ts_tuple_rel_def)
+  qed
+  have lookup_tuple_in': "\<And>as. Mapping.lookup tuple_in' as = safe_max (fst `
+    {tas \<in> ts_tuple_rel (set (linearize data_in)). valid_tuple tuple_since' tas \<and> as = snd tas})"
+  proof -
+    fix as
+    show "Mapping.lookup tuple_in' as = safe_max (fst `
+    {tas \<in> ts_tuple_rel (set (linearize data_in)). valid_tuple tuple_since' tas \<and> as = snd tas})"
+    proof (cases "Mapping.lookup tuple_in as")
+      case None
+      then have "{tas \<in> ts_tuple_rel (set (linearize data_in)).
+        valid_tuple tuple_since tas \<and> as = snd tas} = {}"
+        using valid_before by (auto dest!: safe_max_empty_dest)
+      then have "{tas \<in> ts_tuple_rel (set (linearize data_in)).
+        valid_tuple tuple_since' tas \<and> as = snd tas} = {}"
+        using Mapping_lookup_filter_not_None
+        by (fastforce simp add: valid_tuple_def tuple_since'_def split: option.splits)
+      then show ?thesis
+        unfolding tuple_in_None_None[OF None] using iffD2[OF safe_max_empty, symmetric] by blast
+    next
+      case (Some t)
+      show ?thesis
+      proof (cases "proj_tuple_in_join pos maskL as X")
+        case True
+        then have lookup_tuple_in': "Mapping.lookup tuple_in' as = Some t"
+          using Some unfolding tuple_in'_def by (simp add: Mapping_lookup_filter_Some)
+        have "(t, as) \<in> ts_tuple_rel (set (linearize data_in))" "valid_tuple tuple_since (t, as)"
+          using valid_before Some by (auto dest: safe_max_Some_dest_in[OF finite_fst_ts_tuple_rel])
+        then have t_in_fst: "t \<in> fst ` {tas \<in> ts_tuple_rel (set (linearize data_in)).
+          valid_tuple tuple_since' tas \<and> as = snd tas}"
+          using True by (auto simp add: image_iff valid_tuple_def tuple_since'_def
+            Mapping_lookup_filter_Some split: option.splits)
+        have "\<And>t'. valid_tuple tuple_since' (t', as) \<Longrightarrow> valid_tuple tuple_since (t', as)"
+          using Mapping_lookup_filter_not_None
+          by (fastforce simp add: valid_tuple_def tuple_since'_def split: option.splits)
+        then have "\<And>t'. (t', as) \<in> ts_tuple_rel (set (linearize data_in)) \<Longrightarrow>
+          valid_tuple tuple_since' (t', as) \<Longrightarrow> t' \<le> t"
+          using valid_before Some safe_max_Some_dest_le[OF finite_fst_ts_tuple_rel]
+          by (fastforce simp add: image_iff)
+        then have "Max (fst ` {tas \<in> ts_tuple_rel (set (linearize data_in)).
+          valid_tuple tuple_since' tas \<and> as = snd tas}) = t"
+          using Max_eqI[OF finite_fst_ts_tuple_rel[of "linearize data_in"],
+            OF _ t_in_fst] by fastforce
+        then show ?thesis
+          unfolding lookup_tuple_in' using t_in_fst by (auto simp add: safe_max_def)
+      next
+        case False
+        then have lookup_tuple': "Mapping.lookup tuple_in' as = None"
+          "Mapping.lookup tuple_since' as = None"
+          unfolding tuple_in'_def tuple_since'_def
+          by (auto simp add: Mapping_lookup_filter_None)
+        then have "\<And>tas. \<not>(valid_tuple tuple_since' tas \<and> as = snd tas)"
+          by (auto simp add: valid_tuple_def split: option.splits)
+        then show ?thesis
+          unfolding lookup_tuple' by (auto simp add: safe_max_def)
+      qed
+    qed
+  qed
+  have table_join': "\<And>t ys. (t, ys) \<in> set auxlist \<Longrightarrow> table n R (join ys pos X)"
+  proof -
+    fix t ys
+    assume "(t, ys) \<in> set auxlist"
+    then have table_ys: "table n R ys"
+      using valid_before
+      by (auto simp add: n_def L_def R_def pos_def)
+    show "table n R (join ys pos X)"
+      using join_table[OF table_ys table_left, of pos R] valid_before
+      by (auto simp add: n_def L_def R_def pos_def)
+  qed
+  have table_in': "table n R (Mapping.keys tuple_in')"
+    using tuple_in'_keys valid_before
+    by (auto simp add: n_def L_def R_def pos_def table_def)
+  have table_since': "table n R (Mapping.keys tuple_since')"
+    using tuple_since'_keys valid_before
+    by (auto simp add: n_def L_def R_def pos_def table_def)
+  show ?thesis
+    unfolding join_mmsaux_abs_eq[OF valid_before table_left']
+    using valid_before ts_tuple_rel' lookup_tuple_in' tuple_in'_def tuple_since'_def table_join'
+      Mapping_filter_keys[of tuple_since "\<lambda>as. case as of Some t \<Rightarrow> t \<le> nt"]
+      table_in' table_since' by (auto simp add: n_def L_def R_def pos_def table_def Let_def)
+qed
+
+lemma valid_join_mmsaux: "valid_mmsaux args cur aux auxlist \<Longrightarrow>
+  table (args_n args) (args_L args) X \<Longrightarrow> valid_mmsaux args cur
+  (join_mmsaux args X aux) (map (\<lambda>(t, rel). (t, join rel (args_pos args) X)) auxlist)"
+  using valid_join_mmsaux_unfolded by (cases aux) fast
+
+fun gc_mmsaux :: "'a mmsaux \<Rightarrow> 'a mmsaux" where
+  "gc_mmsaux (nt, gc, maskL, maskR, data_prev, data_in, tuple_in, tuple_since) =
+    (let all_tuples = \<Union>(snd ` (set (linearize data_prev) \<union> set (linearize data_in)));
+    tuple_since' = Mapping.filter (\<lambda>as _. as \<in> all_tuples) tuple_since in
+    (nt, nt, maskL, maskR, data_prev, data_in, tuple_in, tuple_since'))"
+
+lemma valid_gc_mmsaux_unfolded:
+  assumes valid_before: "valid_mmsaux args cur (nt, gc, maskL, maskR, data_prev, data_in,
+    tuple_in, tuple_since) ys"
+  shows "valid_mmsaux args cur (gc_mmsaux (nt, gc, maskL, maskR, data_prev, data_in,
+    tuple_in, tuple_since)) ys"
+proof -
+  define n where "n = args_n args"
+  define L where "L = args_L args"
+  define R where "R = args_R args"
+  define pos where "pos = args_pos args"
+  define all_tuples where "all_tuples \<equiv> \<Union>(snd ` (set (linearize data_prev) \<union>
+    set (linearize data_in)))"
+  define tuple_since' where "tuple_since' \<equiv> Mapping.filter (\<lambda>as _. as \<in> all_tuples) tuple_since"
+  have tuple_since_None_None: "\<And>as. Mapping.lookup tuple_since as = None \<Longrightarrow>
+    Mapping.lookup tuple_since' as = None"
+    unfolding tuple_since'_def using Mapping_lookup_filter_not_None by fastforce
+  have tuple_since'_keys: "\<And>as. as \<in> Mapping.keys tuple_since' \<Longrightarrow> as \<in> Mapping.keys tuple_since"
+    using tuple_since_None_None
+    by (fastforce intro: Mapping_keys_intro dest: Mapping_keys_dest)
+  then have table_since': "table n R (Mapping.keys tuple_since')"
+    using valid_before by (auto simp add: table_def n_def R_def)
+  have data_cong: "\<And>tas. tas \<in> ts_tuple_rel (set (linearize data_prev) \<union>
+    set (linearize data_in)) \<Longrightarrow> valid_tuple tuple_since' tas = valid_tuple tuple_since tas"
+  proof -
+    fix tas
+    assume assm: "tas \<in> ts_tuple_rel (set (linearize data_prev) \<union>
+    set (linearize data_in))"
+    define t where "t \<equiv> fst tas"
+    define as where "as \<equiv> snd tas"
+    have "as \<in> all_tuples"
+      using assm by (force simp add: as_def all_tuples_def ts_tuple_rel_def)
+    then have "Mapping.lookup tuple_since' as = Mapping.lookup tuple_since as"
+      by (auto simp add: tuple_since'_def Mapping.lookup_filter split: option.splits)
+    then show "valid_tuple tuple_since' tas = valid_tuple tuple_since tas"
+      by (auto simp add: valid_tuple_def as_def split: option.splits) metis
+  qed
+  then have data_in_cong: "\<And>tas. tas \<in> ts_tuple_rel (set (linearize data_in)) \<Longrightarrow>
+    valid_tuple tuple_since' tas = valid_tuple tuple_since tas"
+    by (auto simp add: ts_tuple_rel_Un)
+  have "ts_tuple_rel (set ys) =
+    {tas \<in> ts_tuple_rel (set (linearize data_prev) \<union> set (linearize data_in)).
+    valid_tuple tuple_since' tas}"
+    using data_cong valid_before by auto
+  moreover have "(\<forall>as. Mapping.lookup tuple_in as = safe_max (fst `
+    {tas \<in> ts_tuple_rel (set (linearize data_in)). valid_tuple tuple_since' tas \<and> as = snd tas}))"
+    using valid_before by auto (meson data_in_cong)
+  moreover have "(\<forall>as \<in> Mapping.keys tuple_since'. case Mapping.lookup tuple_since' as of
+    Some t \<Rightarrow> t \<le> nt)"
+    using Mapping.keys_filter valid_before
+    by (auto simp add: tuple_since'_def Mapping.lookup_filter split: option.splits
+        intro!: Mapping_keys_intro dest: Mapping_keys_dest)
+  ultimately show ?thesis
+    using all_tuples_def tuple_since'_def valid_before table_since'
+    by (auto simp add: n_def R_def)
+qed
+
+lemma valid_gc_mmsaux: "valid_mmsaux args cur aux ys \<Longrightarrow> valid_mmsaux args cur (gc_mmsaux aux) ys"
+  using valid_gc_mmsaux_unfolded by (cases aux) fast
+
+fun gc_join_mmsaux :: "args \<Rightarrow> 'a table \<Rightarrow> 'a mmsaux \<Rightarrow> 'a mmsaux" where
+  "gc_join_mmsaux args X (t, gc, maskL, maskR, data_prev, data_in, tuple_in, tuple_since) =
+    (if enat (t - gc) > right (args_ivl args) then join_mmsaux args X (gc_mmsaux (t, gc, maskL, maskR,
+      data_prev, data_in, tuple_in, tuple_since))
+    else join_mmsaux args X (t, gc, maskL, maskR, data_prev, data_in, tuple_in, tuple_since))"
+
+lemma gc_join_mmsaux_alt: "gc_join_mmsaux args rel1 aux = join_mmsaux args rel1 (gc_mmsaux aux) \<or>
+  gc_join_mmsaux args rel1 aux = join_mmsaux args rel1 aux"
+  by (cases aux) (auto simp only: gc_join_mmsaux.simps split: if_splits)
+
+lemma valid_gc_join_mmsaux:
+  assumes "valid_mmsaux args cur aux auxlist" "table (args_n args) (args_L args) rel1"
+  shows "valid_mmsaux args cur (gc_join_mmsaux args rel1 aux)
+    (map (\<lambda>(t, rel). (t, join rel (args_pos args) rel1)) auxlist)"
+  using gc_join_mmsaux_alt[of args rel1 aux]
+  using valid_join_mmsaux[OF valid_gc_mmsaux[OF assms(1)] assms(2)]
+    valid_join_mmsaux[OF assms]
+  by auto
+
+fun add_new_table_mmsaux :: "args \<Rightarrow> 'a table \<Rightarrow> 'a mmsaux \<Rightarrow> 'a mmsaux" where
+  "add_new_table_mmsaux args X (t, gc, maskL, maskR, data_prev, data_in, tuple_in, tuple_since) =
     (let tuple_since = upd_set tuple_since (\<lambda>_. t) (X - Mapping.keys tuple_since) in
-    (if 0 \<ge> left I then (t, gc, I, maskL, maskR, data_prev, append_queue (t, X) data_in,
+    (if 0 \<ge> left (args_ivl args) then (t, gc, maskL, maskR, data_prev, append_queue (t, X) data_in,
       upd_set tuple_in (\<lambda>_. t) X, tuple_since)
-    else (t, gc, I, maskL, maskR, append_queue (t, X) data_prev, data_in, tuple_in, tuple_since)))"
+    else (t, gc, maskL, maskR, append_queue (t, X) data_prev, data_in, tuple_in, tuple_since)))"
 
 lemma valid_add_new_table_mmsaux_unfolded:
-  assumes valid_before: "valid_mmsaux w n L R
-    (nt, gc, I, maskL, maskR, data_prev, data_in, tuple_in, tuple_since) auxlist"
-  and table_X: "table n R X"
-  shows "valid_mmsaux w n L R (add_new_table_mmsaux X
-    (nt, gc, I, maskL, maskR, data_prev, data_in, tuple_in, tuple_since))
+  assumes valid_before: "valid_mmsaux args cur
+    (nt, gc, maskL, maskR, data_prev, data_in, tuple_in, tuple_since) auxlist"
+  and table_X: "table (args_n args) (args_R args) X"
+  shows "valid_mmsaux args cur (add_new_table_mmsaux args X
+    (nt, gc, maskL, maskR, data_prev, data_in, tuple_in, tuple_since))
     (case auxlist of
-      [] => [(nt, X)]
-    | ((t, y) # ts) \<Rightarrow> if t = nt then (t, y \<union> X) # ts else (nt, X) # auxlist)"
+      [] => [(cur, X)]
+    | ((t, y) # ts) \<Rightarrow> if t = cur then (t, y \<union> X) # ts else (cur, X) # auxlist)"
 proof -
+  have cur_nt: "cur = nt"
+    using valid_before by auto
+  define I where "I = args_ivl args"
+  define n where "n = args_n args"
+  define L where "L = args_L args"
+  define R where "R = args_R args"
+  define pos where "pos = args_pos args"
   define tuple_in' where "tuple_in' \<equiv> upd_set tuple_in (\<lambda>_. nt) X"
   define tuple_since' where "tuple_since' \<equiv> upd_set tuple_since (\<lambda>_. nt)
     (X - Mapping.keys tuple_since)"
@@ -1104,20 +1231,23 @@ proof -
     [] => [(nt, X)]
     | ((t, y) # ts) \<Rightarrow> if t = nt then (t, y \<union> X) # ts else (nt, X) # auxlist)"
   have table_in': "table n R (Mapping.keys tuple_in')"
-    using table_X valid_before by (auto simp add: table_def tuple_in'_def Mapping_upd_set_keys)
+    using table_X valid_before
+    by (auto simp add: table_def tuple_in'_def Mapping_upd_set_keys n_def R_def)
   have table_since': "table n R (Mapping.keys tuple_since')"
-    using table_X valid_before by (auto simp add: table_def tuple_since'_def Mapping_upd_set_keys)
+    using table_X valid_before
+    by (auto simp add: table_def tuple_since'_def Mapping_upd_set_keys n_def R_def)
   have tuple_since'_keys: "Mapping.keys tuple_since \<subseteq> Mapping.keys tuple_since'"
     using Mapping_upd_set_keys by (fastforce simp add: tuple_since'_def)
   have lin_data_prev': "linearize data_prev' = linearize data_prev @ [(nt, X)]"
     unfolding data_prev'_def append_queue_rep ..
   have wf_data_prev': "\<And>as. as \<in> \<Union>(snd ` (set (linearize data_prev'))) \<Longrightarrow> wf_tuple n R as"
-    unfolding lin_data_prev' using table_X valid_before by (auto simp add: table_def)
+    unfolding lin_data_prev' using table_X valid_before
+    by (auto simp add: table_def n_def R_def)
   have lin_data_in': "linearize data_in' = linearize data_in @ [(nt, X)]"
     unfolding data_in'_def append_queue_rep ..
   have table_auxlist': "\<forall>(t, X) \<in> set auxlist'. table n R X"
     using table_X table_Un valid_before
-    by (auto simp add: auxlist'_def split: list.splits if_splits)
+    by (auto simp add: auxlist'_def n_def R_def split: list.splits if_splits)
   have lookup_tuple_since': "\<forall>as \<in> Mapping.keys tuple_since'.
     case Mapping.lookup tuple_since' as of Some t \<Rightarrow> t \<le> nt"
     unfolding tuple_since'_def using valid_before Mapping_lookup_upd_set[of tuple_since]
@@ -1206,10 +1336,10 @@ proof -
   show ?thesis
   proof (cases "0 \<ge> left I")
     case True
-    then have add_def: "add_new_table_mmsaux X (nt, gc, I, maskL, maskR, data_prev, data_in,
-      tuple_in, tuple_since) = (nt, gc, I, maskL, maskR, data_prev, data_in',
+    then have add_def: "add_new_table_mmsaux args X (nt, gc, maskL, maskR, data_prev, data_in,
+      tuple_in, tuple_since) = (nt, gc, maskL, maskR, data_prev, data_in',
       tuple_in', tuple_since')"
-      using data_in'_def tuple_in'_def tuple_since'_def by auto
+      using data_in'_def tuple_in'_def tuple_since'_def unfolding I_def by auto
     have left_I: "left I = 0"
       using True by auto
     have "\<forall>t \<in> fst ` set (linearize data_in'). t \<le> nt \<and> nt - t \<ge> left I"
@@ -1268,18 +1398,18 @@ proof -
     ultimately show ?thesis
       using assms table_auxlist' sorted_append[of "map fst (linearize data_in)"]
         lookup_tuple_since' ts_tuple_rel_auxlist' table_in' table_since'
-      unfolding add_def auxlist'_def[symmetric]
-      by (auto simp only: valid_mmsaux.simps lin_data_in') auto
+      unfolding add_def auxlist'_def[symmetric] cur_nt I_def
+      by (auto simp only: valid_mmsaux.simps lin_data_in' n_def R_def) auto
   next
     case False
-    then have add_def: "add_new_table_mmsaux X (nt, gc, I, maskL, maskR, data_prev, data_in,
-      tuple_in, tuple_since) = (nt, gc, I, maskL, maskR, data_prev', data_in,
+    then have add_def: "add_new_table_mmsaux args X (nt, gc, maskL, maskR, data_prev, data_in,
+      tuple_in, tuple_since) = (nt, gc, maskL, maskR, data_prev', data_in,
       tuple_in, tuple_since')"
-      using data_prev'_def tuple_since'_def by auto
+      using data_prev'_def tuple_since'_def unfolding I_def by auto
     have left_I: "left I > 0"
       using False by auto
     have "\<forall>t \<in> fst ` set (linearize data_prev'). t \<le> nt \<and> nt - t < left I"
-      using valid_before False by (auto simp add: lin_data_prev')
+      using valid_before False by (auto simp add: lin_data_prev' I_def)
     moreover have "\<And>as. {tas \<in> ts_tuple_rel (set (linearize data_in)).
       valid_tuple tuple_since tas \<and> as = snd tas} =
       {tas \<in> ts_tuple_rel (set (linearize data_in)).
@@ -1300,7 +1430,7 @@ proof -
           using Z_def(4) by (auto simp add: valid_tuple_def tuple_since'_def
               Mapping_lookup_upd_set intro: Mapping_keys_intro split: option.splits if_splits)
         then show ?thesis
-          using Z_def(3) valid_before left_I by auto
+          using Z_def(3) valid_before left_I unfolding I_def by auto
       qed (auto simp add: valid_tuple_def tuple_since'_def Mapping_lookup_upd_set
            dest: Mapping_keys_dest split: option.splits)
     qed (auto simp add: Mapping_lookup_upd_set valid_tuple_def tuple_since'_def
@@ -1309,124 +1439,21 @@ proof -
       using assms table_auxlist' sorted_append[of "map fst (linearize data_prev)"]
         False lookup_tuple_since' ts_tuple_rel_auxlist' table_in' table_since' wf_data_prev'
         valid_before
-      unfolding add_def auxlist'_def[symmetric]
-      by (auto simp only: valid_mmsaux.simps lin_data_prev') fastforce+
+      unfolding add_def auxlist'_def[symmetric] cur_nt I_def
+      by (auto simp only: valid_mmsaux.simps lin_data_prev' n_def R_def) fastforce+
         (* takes long *)
   qed
 qed
 
 lemma valid_add_new_table_mmsaux:
-  assumes valid_before: "valid_mmsaux w n L R aux auxlist"
-  and table_X: "table n R X"
-  and time: "time_mmsaux aux = nt"
-  shows "valid_mmsaux w n L R (add_new_table_mmsaux X aux)
+  assumes valid_before: "valid_mmsaux args cur aux auxlist"
+  and table_X: "table (args_n args) (args_R args) X"
+  shows "valid_mmsaux args cur (add_new_table_mmsaux args X aux)
     (case auxlist of
-      [] => [(nt, X)]
-    | ((t, y) # ts) \<Rightarrow> if t = nt then (t, y \<union> X) # ts else (nt, X) # auxlist)"
-proof -
-  obtain gc I maskL maskR data_prev data_in tuple_in tuple_since where aux_def:
-    "aux = (nt, gc, I, maskL, maskR, data_prev, data_in, tuple_in, tuple_since)"
-    using time by (cases aux) auto
-  show ?thesis
-    using valid_add_new_table_mmsaux_unfolded[OF valid_before[unfolded aux_def] table_X]
-    unfolding aux_def .
-qed
-
-fun gc_mmsaux :: "'a mmsaux \<Rightarrow> 'a mmsaux" where
-  "gc_mmsaux (nt, gc, I, maskL, maskR, data_prev, data_in, tuple_in, tuple_since) =
-    (let all_tuples = \<Union>(snd ` (set (linearize data_prev) \<union> set (linearize data_in)));
-    tuple_since' = Mapping.filter (\<lambda>as _. as \<in> all_tuples) tuple_since in
-    (nt, nt, I, maskL, maskR, data_prev, data_in, tuple_in, tuple_since'))"
-
-lemma valid_gc_mmsaux_unfolded:
-  assumes valid_before: "valid_mmsaux w n L R (nt, gc, I, maskL, maskR, data_prev, data_in,
-    tuple_in, tuple_since) ys"
-  shows "valid_mmsaux w n L R (gc_mmsaux (nt, gc, I, maskL, maskR, data_prev, data_in,
-    tuple_in, tuple_since)) ys"
-proof -
-  define all_tuples where "all_tuples \<equiv> \<Union>(snd ` (set (linearize data_prev) \<union>
-    set (linearize data_in)))"
-  define tuple_since' where "tuple_since' \<equiv> Mapping.filter (\<lambda>as _. as \<in> all_tuples) tuple_since"
-  have tuple_since_None_None: "\<And>as. Mapping.lookup tuple_since as = None \<Longrightarrow>
-    Mapping.lookup tuple_since' as = None"
-    unfolding tuple_since'_def using Mapping_lookup_filter_not_None by fastforce
-  have tuple_since'_keys: "\<And>as. as \<in> Mapping.keys tuple_since' \<Longrightarrow> as \<in> Mapping.keys tuple_since"
-    using tuple_since_None_None
-    by (fastforce intro: Mapping_keys_intro dest: Mapping_keys_dest)
-  then have table_since': "table n R (Mapping.keys tuple_since')"
-    using valid_before by (auto simp add: table_def)
-  have data_cong: "\<And>tas. tas \<in> ts_tuple_rel (set (linearize data_prev) \<union>
-    set (linearize data_in)) \<Longrightarrow> valid_tuple tuple_since' tas = valid_tuple tuple_since tas"
-  proof -
-    fix tas
-    assume assm: "tas \<in> ts_tuple_rel (set (linearize data_prev) \<union>
-    set (linearize data_in))"
-    define t where "t \<equiv> fst tas"
-    define as where "as \<equiv> snd tas"
-    have "as \<in> all_tuples"
-      using assm by (force simp add: as_def all_tuples_def ts_tuple_rel_def)
-    then have "Mapping.lookup tuple_since' as = Mapping.lookup tuple_since as"
-      by (auto simp add: tuple_since'_def Mapping.lookup_filter split: option.splits)
-    then show "valid_tuple tuple_since' tas = valid_tuple tuple_since tas"
-      by (auto simp add: valid_tuple_def as_def split: option.splits) metis
-  qed
-  then have data_in_cong: "\<And>tas. tas \<in> ts_tuple_rel (set (linearize data_in)) \<Longrightarrow>
-    valid_tuple tuple_since' tas = valid_tuple tuple_since tas"
-    by (auto simp add: ts_tuple_rel_Un)
-  have "ts_tuple_rel (set ys) =
-    {tas \<in> ts_tuple_rel (set (linearize data_prev) \<union> set (linearize data_in)).
-    valid_tuple tuple_since' tas}"
-    using data_cong valid_before by auto
-  moreover have "(\<forall>as. Mapping.lookup tuple_in as = safe_max (fst `
-    {tas \<in> ts_tuple_rel (set (linearize data_in)). valid_tuple tuple_since' tas \<and> as = snd tas}))"
-    using valid_before by auto (meson data_in_cong)
-  moreover have "(\<forall>as \<in> Mapping.keys tuple_since'. case Mapping.lookup tuple_since' as of
-    Some t \<Rightarrow> t \<le> nt)"
-    using Mapping.keys_filter valid_before
-    by (auto simp add: tuple_since'_def Mapping.lookup_filter split: option.splits
-        intro!: Mapping_keys_intro dest: Mapping_keys_dest)
-  ultimately show ?thesis
-    using all_tuples_def tuple_since'_def valid_before table_since' by auto
-qed
-
-lemma valid_gc_mmsaux: "valid_mmsaux w n L R aux ys \<Longrightarrow> valid_mmsaux w n L R (gc_mmsaux aux) ys"
-  using valid_gc_mmsaux_unfolded by (cases aux) fast
-
-fun add_new_mmsaux :: "nat \<times> 'a table \<Rightarrow> 'a mmsaux \<Rightarrow> 'a mmsaux" where
-  "add_new_mmsaux (nt, X) (t, gc, I, maskL, maskR, data_prev, data_in, tuple_in, tuple_since) =
-    (if enat (nt - gc) > right I then
-      add_new_table_mmsaux X (add_new_ts_mmsaux nt (gc_mmsaux (t, gc, I, maskL, maskR,
-      data_prev, data_in, tuple_in, tuple_since)))
-    else
-      add_new_table_mmsaux X (add_new_ts_mmsaux nt (t, gc, I, maskL, maskR, data_prev, data_in,
-      tuple_in, tuple_since)))"
-
-lemma valid_add_new_mmsaux_unfolded:
-  assumes valid_before: "valid_mmsaux w n L R
-    (t, gc, I, maskL, maskR, data_prev, data_in, tuple_in, tuple_since) auxlist"
-  and nt_mono: "nt \<ge> current w"
-  and new_window: "w' = w\<lparr>latest := if nt \<ge> left (ivl w) then nt - left (ivl w)
-    else latest w, current := nt\<rparr>"
-  and table_X: "table n R X"
-  shows "valid_mmsaux w' n L R (add_new_mmsaux (nt, X)
-    (t, gc, I, maskL, maskR, data_prev, data_in, tuple_in, tuple_since))
-    (case auxlist of
-      [] => [(nt, X)]
-    | ((t, y) # ts) \<Rightarrow> if t = nt then (t, y \<union> X) # ts else (nt, X) # auxlist)"
-  using valid_add_new_table_mmsaux[OF valid_add_new_ts_mmsaux[OF valid_before nt_mono new_window]
-    table_X]
-    valid_add_new_table_mmsaux[OF valid_add_new_ts_mmsaux[OF valid_gc_mmsaux nt_mono new_window,
-    OF valid_before] table_X]
-  by (auto simp only: valid_mmsaux.simps time_mmsaux.simps add_new_mmsaux.simps
-      add_new_ts_mmsaux.simps gc_mmsaux.simps Let_def split: if_splits prod.splits)
-
-lemma valid_add_new_mmsaux: "valid_mmsaux w n L R aux auxlist \<Longrightarrow> nt \<ge> current w \<Longrightarrow>
-  table n R X \<Longrightarrow> w' = w\<lparr>latest := if nt \<ge> left (ivl w) then nt - left (ivl w)
-  else latest w, current := nt\<rparr> \<Longrightarrow> valid_mmsaux w' n L R (add_new_mmsaux (nt, X) aux)
-  (case auxlist of
-    [] => [(nt, X)]
-  | ((t, y) # ts) \<Rightarrow> if t = nt then (t, y \<union> X) # ts else (nt, X) # auxlist)"
-  using valid_add_new_mmsaux_unfolded by (cases aux) fast
+      [] => [(cur, X)]
+    | ((t, y) # ts) \<Rightarrow> if t = cur then (t, y \<union> X) # ts else (cur, X) # auxlist)"
+  using valid_add_new_table_mmsaux_unfolded assms
+  by (cases aux) fast
 
 lemma foldr_ts_tuple_rel:
   "as \<in> foldr (\<union>) (concat (map (\<lambda>(t, rel). if P t then [rel] else []) auxlist)) {} \<longleftrightarrow>
@@ -1448,34 +1475,34 @@ qed
 lemma image_snd: "(a, b) \<in> X \<Longrightarrow> b \<in> snd ` X"
   by force
 
-fun result_mmsaux :: "'a mmsaux \<Rightarrow> 'a table" where
-  "result_mmsaux (nt, gc, I, maskL, maskR, data_prev, data_in, tuple_in, tuple_since) =
-  Mapping.keys tuple_in"
+fun result_mmsaux :: "args \<Rightarrow> 'a mmsaux \<Rightarrow> 'a table" where
+  "result_mmsaux args (nt, gc, maskL, maskR, data_prev, data_in, tuple_in, tuple_since) =
+    Mapping.keys tuple_in"
 
 lemma valid_result_mmsaux_unfolded:
-  assumes "valid_mmsaux w n L R
-    (t, gc, I, maskL, maskR, data_prev, data_in, tuple_in, tuple_since) auxlist"
-  shows "result_mmsaux (t, gc, I, maskL, maskR, data_prev, data_in, tuple_in, tuple_since) =
-  foldr (\<union>) [rel. (t, rel) \<leftarrow> auxlist, left (ivl w) \<le> current w - t] {}"
+  assumes "valid_mmsaux args cur
+    (t, gc, maskL, maskR, data_prev, data_in, tuple_in, tuple_since) auxlist"
+  shows "result_mmsaux args (t, gc, maskL, maskR, data_prev, data_in, tuple_in, tuple_since) =
+    foldr (\<union>) [rel. (t, rel) \<leftarrow> auxlist, left (args_ivl args) \<le> cur - t] {}"
   using valid_mmsaux_tuple_in_keys[OF assms] assms
-  apply (auto simp add: image_Un ts_tuple_rel_Un foldr_ts_tuple_rel image_snd)
-   apply (fastforce intro!: ts_tuple_rel_intro dest!: ts_tuple_rel_dest)+
-  done
+  by (auto simp add: image_Un ts_tuple_rel_Un foldr_ts_tuple_rel image_snd)
+     (fastforce intro: ts_tuple_rel_intro dest: ts_tuple_rel_dest)+
 
-lemma valid_result_mmsaux: "valid_mmsaux w n L R aux auxlist \<Longrightarrow>
-  result_mmsaux aux = foldr (\<union>) [rel. (t, rel) \<leftarrow> auxlist, left (ivl w) \<le> current w - t] {}"
+lemma valid_result_mmsaux: "valid_mmsaux args cur aux auxlist \<Longrightarrow>
+  result_mmsaux args aux = foldr (\<union>) [rel. (t, rel) \<leftarrow> auxlist, left (args_ivl args) \<le> cur - t] {}"
   using valid_result_mmsaux_unfolded by (cases aux) fast
 
-interpretation default_msaux: msaux valid_mmsaux init_mmsaux filter_mmsaux join_mmsaux
-  add_new_mmsaux result_mmsaux
-  using valid_init_mmsaux valid_filter_mmsaux valid_join_mmsaux valid_add_new_mmsaux
-    valid_result_mmsaux by unfold_locales assumption+
+interpretation default_msaux: msaux valid_mmsaux init_mmsaux add_new_ts_mmsaux gc_join_mmsaux
+  add_new_table_mmsaux result_mmsaux
+  using valid_init_mmsaux valid_add_new_ts_mmsaux valid_gc_join_mmsaux valid_add_new_table_mmsaux
+    valid_result_mmsaux
+  by unfold_locales assumption+
 
 (* optimized until data structure *)
 
 type_synonym tp = nat
 
-type_synonym 'a mmuaux = "tp \<times> nat \<times> ts queue \<times> \<I> \<times> bool \<times> bool list \<times> bool list \<times>
+type_synonym 'a mmuaux = "tp \<times> ts queue \<times> nat \<times> bool list \<times> bool list \<times>
   ('a tuple, tp) mapping \<times> (tp, ('a tuple, ts + tp) mapping) mapping \<times> 'a table list \<times> nat"
 
 definition tstp_lt :: "ts + tp \<Rightarrow> ts \<Rightarrow> tp \<Rightarrow> bool" where
@@ -1551,34 +1578,36 @@ definition filter_a2_map :: "\<I> \<Rightarrow> ts \<Rightarrow> tp \<Rightarrow
 fun triple_eq_pair :: "('a \<times> 'b \<times> 'c) \<Rightarrow> ('a \<times> 'd) \<Rightarrow> ('d \<Rightarrow> 'b) \<Rightarrow> ('a \<Rightarrow> 'd \<Rightarrow> 'c) \<Rightarrow> bool" where
   "triple_eq_pair (t, a1, a2) (ts', tp') f g \<longleftrightarrow> t = ts' \<and> a1 = f tp' \<and> a2 = g ts' tp'"
 
-fun valid_mmuaux' :: "window \<Rightarrow> ts \<Rightarrow> bool \<Rightarrow> nat \<Rightarrow> nat set \<Rightarrow> nat set \<Rightarrow> 'a mmuaux \<Rightarrow> 'a muaux \<Rightarrow>
-  bool" where
-  "valid_mmuaux' w dt b n L R (tp, len, tss, I, pos, maskL, maskR, a1_map, a2_map,
+fun valid_mmuaux' :: "args \<Rightarrow> ts \<Rightarrow> ts \<Rightarrow> 'a mmuaux \<Rightarrow> 'a muaux \<Rightarrow> bool" where
+  "valid_mmuaux' args cur dt (tp, tss, len, maskL, maskR, a1_map, a2_map,
     done, done_length) auxlist \<longleftrightarrow>
-    L \<subseteq> R \<and> maskL = join_mask n L \<and> maskR = join_mask n R \<and> b = pos \<and>
-    I = ivl w \<and> len \<le> tp \<and>
+    args_L args \<subseteq> args_R args \<and>
+    maskL = join_mask (args_n args) (args_L args) \<and>
+    maskR = join_mask (args_n args) (args_R args) \<and>
+    len \<le> tp \<and>
     length (linearize tss) = len \<and> sorted (linearize tss) \<and>
-    (\<forall>t \<in> set (linearize tss). t \<le> current w \<and> enat t + right I \<ge> enat (current w)) \<and>
-    table n L (Mapping.keys a1_map) \<and> Mapping.keys a2_map = {tp - len..tp} \<and>
+    (\<forall>t \<in> set (linearize tss). t \<le> cur \<and> enat cur \<le> enat t + right (args_ivl args)) \<and>
+    table (args_n args) (args_L args) (Mapping.keys a1_map) \<and>
+    Mapping.keys a2_map = {tp - len..tp} \<and>
     (\<forall>xs \<in> Mapping.keys a1_map. case Mapping.lookup a1_map xs of Some tp' \<Rightarrow> tp' < tp) \<and>
     (\<forall>tp' \<in> Mapping.keys a2_map. case Mapping.lookup a2_map tp' of Some m \<Rightarrow>
-      table n R (Mapping.keys m) \<and>
+      table (args_n args) (args_R args) (Mapping.keys m) \<and>
       (\<forall>xs \<in> Mapping.keys m. case Mapping.lookup m xs of Some tstp \<Rightarrow>
-      tstp_lt tstp (current w - (left I - 1)) tp \<and> (isl tstp \<longleftrightarrow> left I > 0))) \<and>
+      tstp_lt tstp (cur - (left (args_ivl args) - 1)) tp \<and> (isl tstp \<longleftrightarrow> left (args_ivl args) > 0))) \<and>
     length done = done_length \<and> length done + len = length auxlist \<and>
     rev done = map proj_thd (take (length done) auxlist) \<and>
-    (\<forall>x \<in> set (take (length done) auxlist). check_before I dt x) \<and>
+    (\<forall>x \<in> set (take (length done) auxlist). check_before (args_ivl args) dt x) \<and>
     sorted (map fst auxlist) \<and>
-    list_all2 (\<lambda>x y. triple_eq_pair x y (\<lambda>tp'. filter_a1_map pos tp' a1_map)
-      (\<lambda>ts' tp'. filter_a2_map I ts' tp' a2_map)) (drop (length done) auxlist)
+    list_all2 (\<lambda>x y. triple_eq_pair x y (\<lambda>tp'. filter_a1_map (args_pos args) tp' a1_map)
+      (\<lambda>ts' tp'. filter_a2_map (args_ivl args) ts' tp' a2_map)) (drop (length done) auxlist)
       (zip (linearize tss) [tp - len..<tp])"
 
-definition valid_mmuaux :: "window \<Rightarrow> bool \<Rightarrow> nat \<Rightarrow> nat set \<Rightarrow> nat set \<Rightarrow> 'a mmuaux \<Rightarrow> 'a muaux \<Rightarrow>
+definition valid_mmuaux :: "args \<Rightarrow> ts \<Rightarrow> 'a mmuaux \<Rightarrow> 'a muaux \<Rightarrow>
   bool" where
-  "valid_mmuaux w = valid_mmuaux' w (current w)"
+  "valid_mmuaux args cur = valid_mmuaux' args cur cur"
 
 fun eval_step_mmuaux :: "'a mmuaux \<Rightarrow> 'a mmuaux" where
-  "eval_step_mmuaux (tp, len, tss, I, pos, maskL, maskR, a1_map, a2_map,
+  "eval_step_mmuaux (tp, tss, len, maskL, maskR, a1_map, a2_map,
     done, done_length) = (case safe_hd tss of (Some ts, tss') \<Rightarrow>
       (case Mapping.lookup a2_map (tp - len) of Some m \<Rightarrow>
         let m = Mapping.filter (\<lambda>_ tstp. ts_tp_lt' ts (tp - len) tstp) m;
@@ -1587,7 +1616,7 @@ fun eval_step_mmuaux :: "'a mmuaux \<Rightarrow> 'a mmuaux" where
           (case Mapping.lookup a2_map (tp - len + 1) of Some m' \<Rightarrow>
           Mapping.combine (\<lambda>tstp tstp'. max_tstp tstp tstp') m m') a2_map;
         a2_map = Mapping.delete (tp - len) a2_map in
-        (tp, len - 1, tl_queue tss', I, pos, maskL, maskR, a1_map, a2_map,
+        (tp, tl_queue tss', len - 1, maskL, maskR, a1_map, a2_map,
         T # done, done_length + 1)))"
 
 lemma Mapping_update_keys: "Mapping.keys (Mapping.update a b m) = Mapping.keys m \<union> {a}"
@@ -1629,24 +1658,27 @@ lemma Mapping_keys_filterD: "k \<in> Mapping.keys (Mapping.filter f m) \<Longrig
   by transfer (auto split: option.splits if_splits)
 
 fun lin_ts_mmuaux :: "'a mmuaux \<Rightarrow> ts list" where
-  "lin_ts_mmuaux (tp, len, tss, I, pos, maskL, maskR, a1_map, a2_map, done, done_length) =
+  "lin_ts_mmuaux (tp, tss, len, maskL, maskR, a1_map, a2_map, done, done_length) =
     linearize tss"
 
 lemma valid_eval_step_mmuaux':
-  assumes "valid_mmuaux' w dt b n L R aux auxlist"
-    "lin_ts_mmuaux aux = ts # tss''" "enat ts + right (ivl w) < dt"
-  shows "valid_mmuaux' w dt b n L R (eval_step_mmuaux aux) auxlist \<and>
+  assumes "valid_mmuaux' args cur dt aux auxlist"
+    "lin_ts_mmuaux aux = ts # tss''" "enat ts + right (args_ivl args) < dt"
+  shows "valid_mmuaux' args cur dt (eval_step_mmuaux aux) auxlist \<and>
     lin_ts_mmuaux (eval_step_mmuaux aux) = tss''"
 proof -
-  obtain tp len tss I pos maskL maskR a1_map a2_map "done" done_length where aux_def:
-    "aux = (tp, len, tss, I, pos, maskL, maskR, a1_map, a2_map, done, done_length)"
+  define I where "I = args_ivl args"
+  define n where "n = args_n args"
+  define L where "L = args_L args"
+  define R where "R = args_R args"
+  define pos where "pos = args_pos args"
+  obtain tp len tss maskL maskR a1_map a2_map "done" done_length where aux_def:
+    "aux = (tp, tss, len, maskL, maskR, a1_map, a2_map, done, done_length)"
     by (cases aux) auto
   then obtain tss' where safe_hd_eq: "safe_hd tss = (Some ts, tss')"
     using assms(2) safe_hd_rep case_optionE
     by (cases "safe_hd tss") fastforce
   note valid_before = assms(1)[unfolded aux_def]
-  have I_ivl_w: "I = ivl w"
-    using valid_before by auto
   have lin_tss_not_Nil: "linearize tss \<noteq> []"
     using safe_hd_rep[OF safe_hd_eq] by auto
   have ts_hd: "ts = hd (linearize tss)"
@@ -1669,12 +1701,12 @@ proof -
     using tp_minus_keys by (auto dest: Mapping_keys_dest)
   have "table n R (Mapping.keys m)"
     "(\<forall>xs \<in> Mapping.keys m. case Mapping.lookup m xs of Some tstp \<Rightarrow>
-    tstp_lt tstp (current w - (left I - 1)) tp \<and> (isl tstp \<longleftrightarrow> left I > 0))"
+    tstp_lt tstp (cur - (left I - 1)) tp \<and> (isl tstp \<longleftrightarrow> left I > 0))"
     using tp_minus_keys m_def valid_before
-    unfolding valid_mmuaux'.simps by fastforce+
+    unfolding valid_mmuaux'.simps n_def I_def R_def by fastforce+
   then have m_inst: "table n R (Mapping.keys m)"
     "\<And>xs tstp. Mapping.lookup m xs = Some tstp \<Longrightarrow>
-    tstp_lt tstp (current w - (left I - 1)) tp \<and> (isl tstp \<longleftrightarrow> left I > 0)"
+    tstp_lt tstp (cur - (left I - 1)) tp \<and> (isl tstp \<longleftrightarrow> left I > 0)"
     using Mapping_keys_intro by fastforce+
   have m_inst_isl: "\<And>xs tstp. Mapping.lookup m xs = Some tstp \<Longrightarrow> isl tstp \<longleftrightarrow> left I > 0"
     using m_inst(2) by fastforce
@@ -1682,12 +1714,12 @@ proof -
     using tp_minus_keys' by (auto dest: Mapping_keys_dest)
   have "table n R (Mapping.keys m')"
     "(\<forall>xs \<in> Mapping.keys m'. case Mapping.lookup m' xs of Some tstp \<Rightarrow>
-    tstp_lt tstp (current w - (left I - 1)) tp \<and> (isl tstp \<longleftrightarrow> left I > 0))"
+    tstp_lt tstp (cur - (left I - 1)) tp \<and> (isl tstp \<longleftrightarrow> left I > 0))"
     using tp_minus_keys' m'_def valid_before
-    unfolding valid_mmuaux'.simps by fastforce+
+    unfolding valid_mmuaux'.simps I_def n_def R_def by fastforce+
   then have m'_inst: "table n R (Mapping.keys m')"
     "\<And>xs tstp. Mapping.lookup m' xs = Some tstp \<Longrightarrow>
-    tstp_lt tstp (current w - (left I - 1)) tp \<and> (isl tstp \<longleftrightarrow> left I > 0)"
+    tstp_lt tstp (cur - (left I - 1)) tp \<and> (isl tstp \<longleftrightarrow> left I > 0)"
     using Mapping_keys_intro by fastforce+
   have m'_inst_isl: "\<And>xs tstp. Mapping.lookup m' xs = Some tstp \<Longrightarrow> isl tstp \<longleftrightarrow> left I > 0"
     using m'_inst(2) by fastforce  
@@ -1697,11 +1729,11 @@ proof -
   define a2_map' where "a2_map' = Mapping.update (tp - len + 1) mc a2_map"
   define a2_map'' where "a2_map'' = Mapping.delete (tp - len) a2_map'"
   have m_upd_lookup: "\<And>xs tstp. Mapping.lookup m_upd xs = Some tstp \<Longrightarrow>
-    tstp_lt tstp (current w - (left I - 1)) tp \<and> (isl tstp \<longleftrightarrow> left I > 0)"
+    tstp_lt tstp (cur - (left I - 1)) tp \<and> (isl tstp \<longleftrightarrow> left I > 0)"
     unfolding m_upd_def Mapping.lookup_filter
     using m_inst(2) by (auto split: option.splits if_splits)
   have mc_lookup: "\<And>xs tstp. Mapping.lookup mc xs = Some tstp \<Longrightarrow>
-    tstp_lt tstp (current w - (left I - 1)) tp \<and> (isl tstp \<longleftrightarrow> left I > 0)"
+    tstp_lt tstp (cur - (left I - 1)) tp \<and> (isl tstp \<longleftrightarrow> left I > 0)"
     unfolding mc_def Mapping.lookup_combine
     using m_upd_lookup m'_inst(2)
     by (auto simp add: combine_options_def max_tstp_isl intro: max_tstp_intro split: option.splits)
@@ -1726,7 +1758,7 @@ proof -
   have list_all2: "list_all2 (\<lambda>x y. triple_eq_pair x y (\<lambda>tp'. filter_a1_map pos tp' a1_map)
     (\<lambda>ts' tp'. filter_a2_map I ts' tp' a2_map))
     (drop (length done) auxlist) (zip (linearize tss) [tp - len..<tp])"
-    using valid_before by auto
+    using valid_before unfolding I_def pos_def by auto
   obtain hd_aux tl_aux where aux_split: "drop (length done) auxlist = hd_aux # tl_aux"
     "case hd_aux of (t, a1, a2) \<Rightarrow> (t, a1, a2) =
     (ts, filter_a1_map pos (tp - len) a1_map, filter_a2_map I ts (tp - len) a2_map)"
@@ -1882,7 +1914,7 @@ proof -
     using filter_a2_map_cong set_tl_tss' by (auto elim!: in_set_zipE split: prod.splits)
   have lookup'': "\<forall>tp' \<in> Mapping.keys a2_map''. case Mapping.lookup a2_map'' tp' of Some m \<Rightarrow>
     table n R (Mapping.keys m) \<and> (\<forall>xs \<in> Mapping.keys m. case Mapping.lookup m xs of Some tstp \<Rightarrow>
-    tstp_lt tstp (current w - (left I - 1)) tp \<and> isl tstp = (0 < left I))"
+    tstp_lt tstp (cur - (left I - 1)) tp \<and> isl tstp = (0 < left I))"
   proof (rule ballI)
     fix tp'
     assume assm: "tp' \<in> Mapping.keys a2_map''"
@@ -1894,7 +1926,7 @@ proof -
       using valid_before by auto
     have "table n R (Mapping.keys f) \<and>
       (\<forall>xs \<in> Mapping.keys f. case Mapping.lookup f xs of Some tstp \<Rightarrow>
-      tstp_lt tstp (current w - (left I - 1)) tp \<and> isl tstp = (0 < left I))"
+      tstp_lt tstp (cur - (left I - 1)) tp \<and> isl tstp = (0 < left I))"
     proof (cases "tp' = tp - (len - 1)")
       case True
       then have f_mc: "f = mc"
@@ -1906,7 +1938,7 @@ proof -
         using mc_keys m_def m'_def m_inst m'_inst
         by (auto simp add: table_def)
       moreover have "\<forall>xs \<in> Mapping.keys f. case Mapping.lookup f xs of Some tstp \<Rightarrow>
-        tstp_lt tstp (current w - (left I - 1)) tp \<and> isl tstp = (0 < left I)"
+        tstp_lt tstp (cur - (left I - 1)) tp \<and> isl tstp = (0 < left I)"
         using assm Mapping.keys_filter m_inst(2) m_inst_isl m'_inst(2) m'_inst_isl max_tstp_isl
         unfolding f_mc mc_def Mapping.lookup_combine
         by (auto simp add: combine_options_def m_upd_def Mapping.lookup_filter
@@ -1920,11 +1952,11 @@ proof -
         using tp'_in id[of tp'] f_def False by auto
       then show ?thesis
         using tp'_in_keys valid_before
-        unfolding valid_mmuaux'.simps by fastforce
+        unfolding valid_mmuaux'.simps I_def n_def R_def by fastforce
     qed
     then show "case Mapping.lookup a2_map'' tp' of Some m \<Rightarrow>
       table n R (Mapping.keys m) \<and> (\<forall>xs \<in> Mapping.keys m. case Mapping.lookup m xs of Some tstp \<Rightarrow>
-      tstp_lt tstp (current w - (left I - 1)) tp \<and> isl tstp = (0 < left I))"
+      tstp_lt tstp (cur - (left I - 1)) tp \<and> isl tstp = (0 < left I))"
       using f_def by auto
   qed
   have tl_aux_def: "tl_aux = drop (length done + 1) auxlist"
@@ -1958,13 +1990,13 @@ proof -
     using valid_before by auto
   then have "\<forall>x \<in> set (take (length done) auxlist). check_before I dt x"
     "rev done = map proj_thd (take (length done) auxlist)"
-    using valid_before by auto
+    using valid_before unfolding I_def by auto
   then have list_all': "(\<forall>x \<in> set (take (length (T # done)) auxlist). check_before I dt x)"
     "rev (T # done) = map proj_thd (take (length (T # done)) auxlist)"
-    using drop_is_Cons_take[OF aux_split(1)] aux_split(2) assms(3)[unfolded I_ivl_w[symmetric]]
-    by (auto simp add: T_eq)
-  have eval_step_mmuaux_eq: "eval_step_mmuaux (tp, len, tss, I, pos, maskL, maskR, a1_map, a2_map,
-    done, done_length) = (tp, len - 1, tl_queue tss', I, pos, maskL, maskR, a1_map, a2_map'',
+    using drop_is_Cons_take[OF aux_split(1)] aux_split(2) assms(3)
+    by (auto simp add: T_eq I_def)
+  have eval_step_mmuaux_eq: "eval_step_mmuaux (tp, tss, len, maskL, maskR, a1_map, a2_map,
+    done, done_length) = (tp, tl_queue tss', len - 1,  maskL, maskR, a1_map, a2_map'',
     T # done, done_length + 1)"
     using safe_hd_eq m_def m'_def m_upd_def T_def mc_def a2_map'_def a2_map''_def
     by (auto simp add: Let_def)
@@ -1972,38 +2004,38 @@ proof -
     using lin_tss_Cons assms(2) unfolding aux_def eval_step_mmuaux_eq by auto
   then show ?thesis
     using valid_before a2_map''_keys sorted_tl list_all' lookup'' list_all2''
-    unfolding eval_step_mmuaux_eq valid_mmuaux'.simps tl_aux_def aux_def
+    unfolding eval_step_mmuaux_eq valid_mmuaux'.simps tl_aux_def aux_def I_def n_def R_def pos_def
     using lin_tss_not_Nil safe_hd_eq len_pos
     by (auto simp add: list.set_sel(2) lin_tss' tl_queue_rep[OF tss'_not_empty] min_auxlist_done)
 qed
 
 lemma done_empty_valid_mmuaux'_intro:
-  assumes "valid_mmuaux' w dt b n L R
-    (tp, len, tss, I, pos, maskL, maskR, a1_map, a2_map, done, done_length) auxlist"
-  shows "valid_mmuaux' w dt' b n L R
-    (tp, len, tss, I, pos, maskL, maskR, a1_map, a2_map, [], 0)
+  assumes "valid_mmuaux' args cur dt
+    (tp, tss, len, maskL, maskR, a1_map, a2_map, done, done_length) auxlist"
+  shows "valid_mmuaux' args cur dt'
+    (tp, tss, len, maskL, maskR, a1_map, a2_map, [], 0)
     (drop (length done) auxlist)"
   using assms sorted_drop by (auto simp add: drop_map[symmetric])
 
 lemma valid_mmuaux'_mono:
-  assumes "valid_mmuaux' w dt b n L R aux auxlist" "dt \<le> dt'"
-  shows "valid_mmuaux' w dt' b n L R aux auxlist"
+  assumes "valid_mmuaux' args cur dt aux auxlist" "dt \<le> dt'"
+  shows "valid_mmuaux' args cur dt' aux auxlist"
   using assms less_le_trans by (cases aux) fastforce
 
 lemma valid_foldl_eval_step_mmuaux':
-  assumes valid_before: "valid_mmuaux' w dt b n L R aux auxlist"
+  assumes valid_before: "valid_mmuaux' args cur dt aux auxlist"
     "lin_ts_mmuaux aux = tss @ tss'"
-    "\<And>ts. ts \<in> set (take (length tss) (lin_ts_mmuaux aux)) \<Longrightarrow> enat ts + right (ivl w) < dt"
-  shows "valid_mmuaux' w dt b n L R (foldl (\<lambda>aux _. eval_step_mmuaux aux) aux tss) auxlist \<and>
+    "\<And>ts. ts \<in> set (take (length tss) (lin_ts_mmuaux aux)) \<Longrightarrow> enat ts + right (args_ivl args) < dt"
+  shows "valid_mmuaux' args cur dt (foldl (\<lambda>aux _. eval_step_mmuaux aux) aux tss) auxlist \<and>
     lin_ts_mmuaux (foldl (\<lambda>aux _. eval_step_mmuaux aux) aux tss) = tss'"
   using assms
 proof (induction tss arbitrary: aux)
   case (Cons ts tss)
   have app_ass: "lin_ts_mmuaux aux = ts # (tss @ tss')"
     using Cons(3) by auto
-  have "enat ts + right (ivl w) < dt"
+  have "enat ts + right (args_ivl args) < dt"
     using Cons by auto
-  then have valid_step: "valid_mmuaux' w dt b n L R (eval_step_mmuaux aux) auxlist"
+  then have valid_step: "valid_mmuaux' args cur dt (eval_step_mmuaux aux) auxlist"
     "lin_ts_mmuaux (eval_step_mmuaux aux) = tss @ tss'"
     using valid_eval_step_mmuaux'[OF Cons(2) app_ass] by auto
   show ?case
@@ -2035,27 +2067,25 @@ proof (induction xs)
   qed auto
 qed auto
 
-fun shift_mmuaux :: "ts \<Rightarrow> 'a mmuaux \<Rightarrow> 'a mmuaux" where
-  "shift_mmuaux nt (tp, len, tss, I, pos, maskL, maskR, a1_map, a2_map, done, done_length) =
-    (let tss_list = linearize (takeWhile_queue (\<lambda>t. enat t + right I < enat nt) tss) in
-    foldl (\<lambda>aux _. eval_step_mmuaux aux) (tp, len, tss, I, pos, maskL, maskR,
+fun shift_mmuaux :: "args \<Rightarrow> ts \<Rightarrow> 'a mmuaux \<Rightarrow> 'a mmuaux" where
+  "shift_mmuaux args nt (tp, tss, len, maskL, maskR, a1_map, a2_map, done, done_length) =
+    (let tss_list = linearize (takeWhile_queue (\<lambda>t. enat t + right (args_ivl args) < enat nt) tss) in
+    foldl (\<lambda>aux _. eval_step_mmuaux aux) (tp, tss, len, maskL, maskR,
       a1_map, a2_map, done, done_length) tss_list)"
 
 lemma valid_shift_mmuaux':
-  assumes "valid_mmuaux' w (current w) b n L R aux auxlist" "nt \<ge> current w"
-  shows "valid_mmuaux' w nt b n L R (shift_mmuaux nt aux) auxlist \<and>
-    (\<forall>ts \<in> set (lin_ts_mmuaux (shift_mmuaux nt aux)). \<not>enat ts + right (ivl w) < nt)"
+  assumes "valid_mmuaux' args cur cur aux auxlist" "nt \<ge> cur"
+  shows "valid_mmuaux' args cur nt (shift_mmuaux args nt aux) auxlist \<and>
+    (\<forall>ts \<in> set (lin_ts_mmuaux (shift_mmuaux args nt aux)). \<not>enat ts + right (args_ivl args) < nt)"
 proof -
-  have valid_folded: "valid_mmuaux' w nt b n L R aux auxlist"
+  define I where "I = args_ivl args"
+  define pos where "pos = args_pos args"
+  have valid_folded: "valid_mmuaux' args cur nt aux auxlist"
     using assms(1,2) valid_mmuaux'_mono unfolding valid_mmuaux_def by blast
-  obtain tp len tss I pos maskL maskR a1_map a2_map "done" done_length where aux_def:
-    "aux = (tp, len, tss, I, pos, maskL, maskR, a1_map, a2_map, done, done_length)"
+  obtain tp len tss maskL maskR a1_map a2_map "done" done_length where aux_def:
+    "aux = (tp, tss, len, maskL, maskR, a1_map, a2_map, done, done_length)"
     by (cases aux) auto
-  have b_pos: "b = pos"
-    using valid_folded unfolding aux_def by auto
-  note valid_before = valid_folded[unfolded aux_def this]
-  have I_ivl_w: "I = ivl w"
-    using valid_before by auto
+  note valid_before = valid_folded[unfolded aux_def]
   define tss_list where "tss_list =
     linearize (takeWhile_queue (\<lambda>t. enat t + right I < enat nt) tss)"
   have tss_list_takeWhile: "tss_list = takeWhile (\<lambda>t. enat t + right I < enat nt) (linearize tss)"
@@ -2063,26 +2093,26 @@ proof -
   then obtain tss_list' where tss_list'_def: "linearize tss = tss_list @ tss_list'"
     "tss_list' = dropWhile (\<lambda>t. enat t + right I < enat nt) (linearize tss)"
     by auto
-  obtain tp' len' tss' I' pos' maskL' maskR' a1_map' a2_map' "done'" done_length' where
-    foldl_aux_def: "(tp', len', tss', I', pos', maskL', maskR', a1_map', a2_map',
+  obtain tp' len' tss' maskL' maskR' a1_map' a2_map' "done'" done_length' where
+    foldl_aux_def: "(tp', tss', len', maskL', maskR', a1_map', a2_map',
       done', done_length') = foldl (\<lambda>aux _. eval_step_mmuaux aux) aux tss_list"
     by (cases "foldl (\<lambda>aux _. eval_step_mmuaux aux) aux tss_list") auto
   have lin_tss_aux: "lin_ts_mmuaux aux = linearize tss"
     unfolding aux_def by auto
   have "take (length tss_list) (lin_ts_mmuaux aux) = tss_list"
     unfolding lin_tss_aux using tss_list'_def(1) by auto
-  then have valid_foldl: "valid_mmuaux' w nt pos n L R
+  then have valid_foldl: "valid_mmuaux' args cur nt
     (foldl (\<lambda>aux _. eval_step_mmuaux aux) aux tss_list) auxlist"
     "lin_ts_mmuaux (foldl (\<lambda>aux _. eval_step_mmuaux aux) aux tss_list) = tss_list'"
     using valid_foldl_eval_step_mmuaux'[OF valid_before[folded aux_def], unfolded lin_tss_aux,
-      OF tss_list'_def(1)] tss_list_takeWhile I_ivl_w set_takeWhileD
-    unfolding lin_tss_aux by fastforce+
-  have shift_mmuaux_eq: "shift_mmuaux nt aux = foldl (\<lambda>aux _. eval_step_mmuaux aux) aux tss_list"
-    using tss_list_def unfolding aux_def by auto
-  have "\<And>ts. ts \<in> set tss_list' \<Longrightarrow> \<not>enat ts + right (ivl w) < nt"
-    using sorted_dropWhile_filter tss_list'_def(2) valid_before unfolding I_ivl_w by auto
+      OF tss_list'_def(1)] tss_list_takeWhile set_takeWhileD
+    unfolding lin_tss_aux I_def by fastforce+
+  have shift_mmuaux_eq: "shift_mmuaux args nt aux = foldl (\<lambda>aux _. eval_step_mmuaux aux) aux tss_list"
+    using tss_list_def unfolding aux_def I_def by auto
+  have "\<And>ts. ts \<in> set tss_list' \<Longrightarrow> \<not>enat ts + right (args_ivl args) < nt"
+    using sorted_dropWhile_filter tss_list'_def(2) valid_before unfolding I_def by auto
   then show ?thesis
-    using valid_foldl(1)[unfolded shift_mmuaux_eq[symmetric] b_pos[symmetric]]
+    using valid_foldl(1)[unfolded shift_mmuaux_eq[symmetric]]
     unfolding valid_foldl(2)[unfolded shift_mmuaux_eq[symmetric]] by auto
 qed
 
@@ -2112,10 +2142,11 @@ lemma upd_nested_keys: "Mapping.keys (upd_nested m d f X) = Mapping.keys m \<uni
   by (auto simp add: upd_nested_lookup Domain.DomainI fst_eq_Domain intro!: Mapping_keys_intro
       dest!: Mapping_keys_dest split: option.splits)
 
-fun add_new_mmuaux :: "'a table \<Rightarrow> 'a table \<Rightarrow> ts \<Rightarrow> 'a mmuaux \<Rightarrow> 'a mmuaux" where
-  "add_new_mmuaux rel1 rel2 nt aux =
-    (let (tp, len, tss, I, pos, maskL, maskR, a1_map, a2_map, done, done_length) =
-    shift_mmuaux nt aux;
+fun add_new_mmuaux :: "args \<Rightarrow> 'a table \<Rightarrow> 'a table \<Rightarrow> ts \<Rightarrow> 'a mmuaux \<Rightarrow> 'a mmuaux" where
+  "add_new_mmuaux args rel1 rel2 nt aux =
+    (let (tp, tss, len, maskL, maskR, a1_map, a2_map, done, done_length) =
+    shift_mmuaux args nt aux;
+    I = args_ivl args; pos = args_pos args;
     new_tstp = (if left I = 0 then Inr tp else Inl (nt - (left I - 1)));
     tmp = \<Union>((\<lambda>as. case Mapping.lookup a1_map (proj_tuple maskL as) of None \<Rightarrow>
       (if \<not>pos then {(tp - len, as)} else {})
@@ -2126,7 +2157,7 @@ fun add_new_mmuaux :: "'a table \<Rightarrow> 'a table \<Rightarrow> ts \<Righta
     a1_map = (if pos then Mapping.filter (\<lambda>as _. as \<in> rel1)
       (upd_set a1_map (\<lambda>_. tp) (rel1 - Mapping.keys a1_map)) else upd_set a1_map (\<lambda>_. tp) rel1);
     tss = append_queue nt tss in
-    (tp + 1, len + 1, tss, I, pos, maskL, maskR, a1_map, a2_map, done, done_length))"
+    (tp + 1, tss, len + 1, maskL, maskR, a1_map, a2_map, done, done_length))"
 
 lemma fst_case: "(\<lambda>x. fst (case x of (t, a1, a2) \<Rightarrow> (t, y t a1 a2, z t a1 a2))) = fst"
   by auto
@@ -2153,27 +2184,27 @@ lemma take_length_takeWhile: "length xs \<le> length ys \<Longrightarrow>
       not_less_eq_eq takeWhile_eq_all_conv takeWhile_tail take_Suc_conv_app_nth)
 
 lemma valid_add_new_mmuaux:
-  assumes valid_before: "valid_mmuaux w b n L R aux auxlist"
-    and tabs: "table n L rel1" "table n R rel2"
-    and nt_mono: "nt \<ge> current w"
-    and new_window: "w' = w\<lparr>current := nt\<rparr>"
-  shows "valid_mmuaux w' b n L R (add_new_mmuaux rel1 rel2 nt aux)
-    (update_until (ivl w) b rel1 rel2 nt auxlist)"
+  assumes valid_before: "valid_mmuaux args cur aux auxlist"
+    and tabs: "table (args_n args) (args_L args) rel1" "table (args_n args) (args_R args) rel2"
+    and nt_mono: "nt \<ge> cur"
+  shows "valid_mmuaux args nt (add_new_mmuaux args rel1 rel2 nt aux)
+    (update_until args rel1 rel2 nt auxlist)"
 proof -
-  have valid_folded: "valid_mmuaux' w nt b n L R aux auxlist"
+  define I where "I = args_ivl args"
+  define n where "n = args_n args"
+  define L where "L = args_L args"
+  define R where "R = args_R args"
+  define pos where "pos = args_pos args"
+  have valid_folded: "valid_mmuaux' args cur nt aux auxlist"
     using assms(1,4) valid_mmuaux'_mono unfolding valid_mmuaux_def by blast
-  obtain tp len tss I pos maskL maskR a1_map a2_map "done" done_length where shift_aux_def:
-    "shift_mmuaux nt aux = (tp, len, tss, I, pos, maskL, maskR, a1_map, a2_map, done, done_length)"
-    by (cases "shift_mmuaux nt aux") auto
-  have valid_shift_aux: "valid_mmuaux' w nt b n L R (tp, len, tss, I, pos, maskL, maskR,
+  obtain tp len tss maskL maskR a1_map a2_map "done" done_length where shift_aux_def:
+    "shift_mmuaux args nt aux = (tp, tss, len, maskL, maskR, a1_map, a2_map, done, done_length)"
+    by (cases "shift_mmuaux args nt aux") auto
+  have valid_shift_aux: "valid_mmuaux' args cur nt (tp, tss, len, maskL, maskR,
     a1_map, a2_map, done, done_length) auxlist"
-    "\<And>ts. ts \<in> set (linearize tss) \<Longrightarrow> \<not>enat ts + right (ivl w) < enat nt"
+    "\<And>ts. ts \<in> set (linearize tss) \<Longrightarrow> \<not>enat ts + right (args_ivl args) < enat nt"
     using valid_shift_mmuaux'[OF assms(1)[unfolded valid_mmuaux_def] assms(4)]
     unfolding shift_aux_def by auto
-  have b_pos: "b = pos"
-    using valid_shift_aux unfolding shift_aux_def by auto
-  have I_ivl_w: "I = ivl w"
-    using valid_shift_aux by auto
   define new_tstp where "new_tstp = (if left I = 0 then Inr tp else Inl (nt - (left I - 1)))"
   have new_tstp_lt_isl: "tstp_lt new_tstp (nt - (left I - 1)) (tp + 1)"
     "isl new_tstp \<longleftrightarrow> left I > 0"
@@ -2187,22 +2218,23 @@ proof -
   then have fst_tmp: "\<And>tp'. tp' \<in> fst ` tmp \<Longrightarrow> tp - len \<le> tp' \<and> tp' < tp + 1"
     unfolding tmp_def by (auto simp add: less_SucI split: option.splits if_splits)
   have snd_tmp: "\<And>tp'. table n R (snd ` tmp)"
-    using tabs(2) unfolding tmp_def
+    using tabs(2) unfolding tmp_def n_def R_def
     by (auto simp add: table_def split: if_splits option.splits)
   define a2_map' where "a2_map' = Mapping.update (tp + 1) Mapping.empty
     (upd_nested a2_map new_tstp (max_tstp new_tstp) tmp)"
   define a1_map' where "a1_map' = (if pos then Mapping.filter (\<lambda>as _. as \<in> rel1)
     (upd_set a1_map (\<lambda>_. tp) (rel1 - Mapping.keys a1_map)) else upd_set a1_map (\<lambda>_. tp) rel1)"
   define tss' where "tss' = append_queue nt tss"
-  have add_new_mmuaux_eq: "add_new_mmuaux rel1 rel2 nt aux = (tp + 1, len + 1, tss', I, pos,
+  have add_new_mmuaux_eq: "add_new_mmuaux args rel1 rel2 nt aux = (tp + 1, tss', len + 1,
     maskL, maskR, a1_map', a2_map', done, done_length)"
     using shift_aux_def new_tstp_def tmp_def a2_map'_def a1_map'_def tss'_def
+    unfolding I_def pos_def
     by (auto simp only: add_new_mmuaux.simps Let_def)
-  have update_until_eq: "update_until I pos rel1 rel2 nt auxlist =
+  have update_until_eq: "update_until args rel1 rel2 nt auxlist =
     (map (\<lambda>x. case x of (t, a1, a2) \<Rightarrow> (t, if pos then join a1 True rel1 else a1 \<union> rel1,
       if mem (nt - t) I then a2 \<union> join rel2 pos a1 else a2)) auxlist) @
     [(nt, rel1, if left I = 0 then rel2 else empty_table)]"
-    unfolding update_until_def by simp
+    unfolding update_until_def I_def pos_def by simp
   have len_done_auxlist: "length done \<le> length auxlist"
     using valid_shift_aux by auto
   have auxlist_split: "auxlist = take (length done) auxlist @ drop (length done) auxlist"
@@ -2211,22 +2243,22 @@ proof -
     unfolding tss'_def append_queue_rep by (rule refl)
   have len_lin_tss': "length (linearize tss') = len + 1"
     unfolding lin_tss' using valid_shift_aux by auto
-  have tmp: "sorted (linearize tss)" "\<And>t. t \<in> set (linearize tss) \<Longrightarrow> t \<le> current w"
+  have tmp: "sorted (linearize tss)" "\<And>t. t \<in> set (linearize tss) \<Longrightarrow> t \<le> cur"
     using valid_shift_aux by auto
   have sorted_lin_tss': "sorted (linearize tss')"
     unfolding lin_tss' using tmp(1) le_trans[OF _ assms(4), OF tmp(2)]
     by (simp add: sorted_append)
   have in_lin_tss: "\<And>t. t \<in> set (linearize tss) \<Longrightarrow>
-    t \<le> current w \<and> enat (current w) \<le> enat t + right I"
-    using valid_shift_aux(1) by auto
+    t \<le> cur \<and> enat cur \<le> enat t + right I"
+    using valid_shift_aux(1) unfolding I_def by auto
   then have set_lin_tss': "\<forall>t \<in> set (linearize tss'). t \<le> nt \<and> enat nt \<le> enat t + right I"
-    unfolding lin_tss' I_ivl_w using le_trans[OF _ assms(4)] valid_shift_aux(2)
+    unfolding lin_tss' I_def using le_trans[OF _ assms(4)] valid_shift_aux(2)
     by (auto simp add: not_less)
   have a1_map'_keys: "Mapping.keys a1_map' \<subseteq> Mapping.keys a1_map \<union> rel1"
     unfolding a1_map'_def using Mapping.keys_filter Mapping_upd_set_keys
     by (auto simp add: Mapping_upd_set_keys split: if_splits dest: Mapping_keys_filterD)
   then have tab_a1_map'_keys: "table n L (Mapping.keys a1_map')"
-    using valid_shift_aux(1) tabs(1) by (auto simp add: table_def)
+    using valid_shift_aux(1) tabs(1) by (auto simp add: table_def n_def L_def)
   have a2_map_keys: "Mapping.keys a2_map = {tp - len..tp}"
     using valid_shift_aux by auto
   have a2_map'_keys: "Mapping.keys a2_map' = {tp - len..tp + 1}"
@@ -2234,35 +2266,35 @@ proof -
     by fastforce
   then have a2_map'_keys': "Mapping.keys a2_map' = {tp + 1 - (len + 1)..tp + 1}"
     by auto
-  have len_upd_until: "length done + (len + 1) = length (update_until I pos rel1 rel2 nt auxlist)"
+  have len_upd_until: "length done + (len + 1) = length (update_until args rel1 rel2 nt auxlist)"
     using valid_shift_aux unfolding update_until_eq by auto
   have set_take_auxlist: "\<And>x. x \<in> set (take (length done) auxlist) \<Longrightarrow> check_before I nt x"
-    using valid_shift_aux by auto
+    using valid_shift_aux unfolding I_def by auto
   have list_all2_triple: "list_all2 (\<lambda>x y. triple_eq_pair x y (\<lambda>tp'. filter_a1_map pos tp' a1_map)
     (\<lambda>ts' tp'. filter_a2_map I ts' tp' a2_map)) (drop (length done) auxlist)
     (zip (linearize tss) [tp - len..<tp])"
-    using valid_shift_aux by auto
+    using valid_shift_aux unfolding I_def pos_def by auto
   have set_drop_auxlist: "\<And>x. x \<in> set (drop (length done) auxlist) \<Longrightarrow> \<not>check_before I nt x"
     using valid_shift_aux(2)[OF list_all2_zip[OF list_all2_triple,
       of "\<lambda>y. y \<in> set (linearize tss)"]]
-    unfolding I_ivl_w by auto
+    unfolding I_def by auto
   have length_done_auxlist: "length done \<le> length auxlist"
     using valid_shift_aux by auto
   have take_auxlist_takeWhile: "take (length done) auxlist = takeWhile (check_before I nt) auxlist"
     using take_length_takeWhile[OF length_done_auxlist set_take_auxlist set_drop_auxlist] .
-  have set_take_auxlist': "\<And>x. x \<in> set (take (length done)
-    (update_until I pos rel1 rel2 nt auxlist)) \<Longrightarrow> check_before I nt x"
-    by (metis (no_types, lifting) add_right_cancel auxlist_split length_append length_done_auxlist
-        length_drop length_map map_proj_thd_update_until
-        ordered_cancel_comm_monoid_diff_class.add_diff_inverse set_takeWhileD
-        takeWhile_eq_take take_auxlist_takeWhile)
+  have "length done = length (takeWhile (check_before I nt) auxlist)"
+    by (metis (no_types) add_diff_cancel_right' auxlist_split diff_diff_cancel
+        length_append length_done_auxlist length_drop take_auxlist_takeWhile)
+  then have set_take_auxlist': "\<And>x. x \<in> set (take (length done)
+    (update_until args rel1 rel2 nt auxlist)) \<Longrightarrow> check_before I nt x"
+    by (metis I_def length_map map_proj_thd_update_until set_takeWhileD takeWhile_eq_take)
   have rev_done: "rev done = map proj_thd (take (length done) auxlist)"
     using valid_shift_aux by auto
   moreover have "\<dots> = map proj_thd (takeWhile (check_before I nt)
-    (update_until I pos rel1 rel2 nt auxlist))"
-    by (simp add: take_auxlist_takeWhile map_proj_thd_update_until)
+    (update_until args rel1 rel2 nt auxlist))"
+    by (simp add: take_auxlist_takeWhile map_proj_thd_update_until I_def)
   finally have rev_done': "rev done = map proj_thd (take (length done)
-    (update_until I pos rel1 rel2 nt auxlist))"
+    (update_until args rel1 rel2 nt auxlist))"
     by (metis length_map length_rev takeWhile_eq_take)
   have map_fst_auxlist_take: "\<And>t. t \<in> set (map fst (take (length done) auxlist)) \<Longrightarrow> t \<le> nt"
     using set_take_auxlist
@@ -2298,14 +2330,14 @@ proof -
     using lookup_a1_map_keys unfolding a1_map'_def
     by (auto simp add: Mapping.lookup_filter Mapping_lookup_upd_set Mapping_upd_set_keys
         split: option.splits dest: Mapping_keys_dest) fastforce+
-  have sorted_upd_until: "sorted (map fst (update_until I pos rel1 rel2 nt auxlist))"
+  have sorted_upd_until: "sorted (map fst (update_until args rel1 rel2 nt auxlist))"
     using sorted_fst_auxlist set_map_fst_auxlist
     unfolding update_until_eq
     by (auto simp add: sorted_append comp_def fst_case)
   have lookup_a2_map: "\<And>tp' m. Mapping.lookup a2_map tp' = Some m \<Longrightarrow>
     table n R (Mapping.keys m) \<and> (\<forall>xs \<in> Mapping.keys m. case Mapping.lookup m xs of Some tstp \<Rightarrow>
-      tstp_lt tstp (current w - (left I - 1)) tp \<and> (isl tstp \<longleftrightarrow> left I > 0))"
-    using valid_shift_aux(1) Mapping_keys_intro by force
+      tstp_lt tstp (cur - (left I - 1)) tp \<and> (isl tstp \<longleftrightarrow> left I > 0))"
+    using valid_shift_aux(1) Mapping_keys_intro unfolding I_def n_def R_def by force
   then have lookup_a2_map': "\<And>tp' m xs tstp. Mapping.lookup a2_map tp' = Some m \<Longrightarrow>
     Mapping.lookup m xs = Some tstp \<Longrightarrow> tstp_lt tstp (nt - (left I - 1)) tp \<and>
     isl tstp = (0 < left I)"
@@ -2391,7 +2423,7 @@ proof -
     map (\<lambda>x. case x of (t, a1, a2) \<Rightarrow> (t, if pos then join a1 True rel1 else a1 \<union> rel1,
       if left I \<le> nt - t then a2 \<union> join rel2 pos a1 else a2)) (drop (length done) auxlist)"
     using set_drop_auxlist_cong by auto
-  have "drop (length done) (update_until I pos rel1 rel2 nt auxlist) =
+  have "drop (length done) (update_until args rel1 rel2 nt auxlist) =
     map (\<lambda>x. case x of (t, a1, a2) \<Rightarrow> (t, if pos then join a1 True rel1 else a1 \<union> rel1,
       if mem (nt - t) I then a2 \<union> join rel2 pos a1 else a2)) (drop (length done) auxlist) @
     [(nt, rel1, if left I = 0 then rel2 else empty_table)]"
@@ -2431,13 +2463,14 @@ proof -
     then have t_nt: "t \<le> nt"
       unfolding eqs(1) .
     have "table n L (Mapping.keys a1_map)"
-      using valid_shift_aux by auto
+      using valid_shift_aux unfolding n_def L_def by auto
     then have a1_tab: "table n L a1"
       unfolding eqs(2) filter_a1_map_def by (auto simp add: table_def)
+    note tabR = tabs(2)[unfolded n_def[symmetric] R_def[symmetric]]
     have join_rel2_assms: "L \<subseteq> R" "maskL = join_mask n L"
-      using valid_shift_aux by auto
+      using valid_shift_aux unfolding n_def L_def R_def by auto
     have join_rel2_eq: "join rel2 pos a1 = {xs \<in> rel2. proj_tuple_in_join pos maskL xs a1}"
-      using join_sub[OF join_rel2_assms(1) a1_tab tabs(2)] join_rel2_assms(2) by auto
+      using join_sub[OF join_rel2_assms(1) a1_tab tabR] join_rel2_assms(2) by auto
     have filter_sub_a2: "\<And>xs m' tp'' tstp. tp'' \<le> tp' \<Longrightarrow>
       Mapping.lookup a2_map' tp'' = Some m' \<Longrightarrow> Mapping.lookup m' xs = Some tstp \<Longrightarrow>
       ts_tp_lt' ts' tp' tstp \<Longrightarrow> (tstp = new_tstp \<Longrightarrow> False) \<Longrightarrow>
@@ -2533,8 +2566,9 @@ proof -
     have "pos \<Longrightarrow> filter_a1_map pos tp' a1_map' = join a1 True rel1"
     proof -
       assume pos: pos
+      note tabL = tabs(1)[unfolded n_def[symmetric] L_def[symmetric]]
       have join_eq: "join a1 True rel1 = a1 \<inter> rel1"
-        using join_eq[OF tabs(1) a1_tab] by auto
+        using join_eq[OF tabL a1_tab] by auto
       show "filter_a1_map pos tp' a1_map' = join a1 True rel1"
         using eqs(2) pos tp'_lt_tp unfolding filter_a1_map_def a1_map'_def join_eq
         apply (auto simp add: Mapping.lookup_filter Mapping_lookup_upd_set
@@ -2933,22 +2967,17 @@ proof -
     using valid_shift_aux(1) by auto
   have list_all2': "list_all2 (\<lambda>x y. triple_eq_pair x y (\<lambda>tp'. filter_a1_map pos tp' a1_map')
     (\<lambda>ts' tp'. filter_a2_map I ts' tp' a2_map'))
-    (drop (length done) (update_until I pos rel1 rel2 nt auxlist))
+    (drop (length done) (update_until args rel1 rel2 nt auxlist))
     (zip (linearize tss') [tp + 1 - (len + 1)..<tp + 1])"
     unfolding lin_tss' tp_upt_Suc drop_update_until zip_dist
     using filter_a1_map_rel1 filter_a1_map_rel2 list_all2_appendI[OF list_all2_old]
     by auto
-  have cur_w': "current w' = nt"
-    using assms(5) by auto
-  have ivl_w': "ivl w' = I"
-    using assms(5) I_ivl_w by auto
   show ?thesis
     using valid_shift_aux len_lin_tss' sorted_lin_tss' set_lin_tss' tab_a1_map'_keys a2_map'_keys'
       len_upd_until sorted_upd_until lookup_a1_map_keys' rev_done' set_take_auxlist'
       lookup_a2_map'_keys list_all2'
-    unfolding valid_mmuaux_def add_new_mmuaux_eq valid_mmuaux'.simps I_ivl_w[symmetric] ivl_w'
-      cur_w' b_pos
-    by auto
+    unfolding valid_mmuaux_def add_new_mmuaux_eq valid_mmuaux'.simps
+      I_def n_def L_def R_def pos_def by auto
 qed
 
 lemma list_all2_check_before: "list_all2 (\<lambda>x y. triple_eq_pair x y f g) xs (zip ys zs) \<Longrightarrow>
@@ -2958,71 +2987,70 @@ lemma list_all2_check_before: "list_all2 (\<lambda>x y. triple_eq_pair x y f g) 
    apply (metis in_set_zipE list.set_intros(1))
   by (metis set_subset_Cons subsetD zip_eq_ConsE)
 
-fun eval_mmuaux :: "ts \<Rightarrow> 'a mmuaux \<Rightarrow> 'a table list \<times> 'a mmuaux" where
-  "eval_mmuaux nt aux =
-    (let (tp, len, tss, I, pos, maskL, maskR, a1_map, a2_map, done, done_length) =
-    shift_mmuaux nt aux in
-    (rev done, (tp, len, tss, I, pos, maskL, maskR, a1_map, a2_map, [], 0)))"
+fun eval_mmuaux :: "args \<Rightarrow> ts \<Rightarrow> 'a mmuaux \<Rightarrow> 'a table list \<times> 'a mmuaux" where
+  "eval_mmuaux args nt aux =
+    (let (tp, tss, len, maskL, maskR, a1_map, a2_map, done, done_length) =
+    shift_mmuaux args nt aux in
+    (rev done, (tp, tss, len, maskL, maskR, a1_map, a2_map, [], 0)))"
 
 lemma valid_eval_mmuaux:
-  assumes "valid_mmuaux w b n L R aux auxlist" "nt \<ge> current w"
-    "eval_mmuaux nt aux = (res, aux')" "eval_until (ivl w) nt auxlist = (res', auxlist')"
-  shows "res = res' \<and> valid_mmuaux w b n L R aux' auxlist'"
+  assumes "valid_mmuaux args cur aux auxlist" "nt \<ge> cur"
+    "eval_mmuaux args nt aux = (res, aux')" "eval_until (args_ivl args) nt auxlist = (res', auxlist')"
+  shows "res = res' \<and> valid_mmuaux args cur aux' auxlist'"
 proof -
-  have valid_folded: "valid_mmuaux' w nt b n L R aux auxlist"
+  define I where "I = args_ivl args"
+  define pos where "pos = args_pos args"
+  have valid_folded: "valid_mmuaux' args cur nt aux auxlist"
     using assms(1,2) valid_mmuaux'_mono unfolding valid_mmuaux_def by blast
-  obtain tp len tss I pos maskL maskR a1_map a2_map "done" done_length where shift_aux_def:
-    "shift_mmuaux nt aux = (tp, len, tss, I, pos, maskL, maskR, a1_map, a2_map, done, done_length)"
-    by (cases "shift_mmuaux nt aux") auto
-  have valid_shift_aux: "valid_mmuaux' w nt b n L R (tp, len, tss, I, pos, maskL, maskR,
+  obtain tp len tss maskL maskR a1_map a2_map "done" done_length where shift_aux_def:
+    "shift_mmuaux args nt aux = (tp, tss, len, maskL, maskR, a1_map, a2_map, done, done_length)"
+    by (cases "shift_mmuaux args nt aux") auto
+  have valid_shift_aux: "valid_mmuaux' args cur nt (tp, tss, len, maskL, maskR,
     a1_map, a2_map, done, done_length) auxlist"
-    "\<And>ts. ts \<in> set (linearize tss) \<Longrightarrow> \<not>enat ts + right (ivl w) < enat nt"
+    "\<And>ts. ts \<in> set (linearize tss) \<Longrightarrow> \<not>enat ts + right (args_ivl args) < enat nt"
     using valid_shift_mmuaux'[OF assms(1)[unfolded valid_mmuaux_def] assms(2)]
     unfolding shift_aux_def by auto
-  have b_pos: "b = pos"
-    using valid_shift_aux unfolding shift_aux_def by auto
-  have I_ivl_w: "I = ivl w"
-    using valid_shift_aux by auto
   have len_done_auxlist: "length done \<le> length auxlist"
     using valid_shift_aux by auto
   have list_all: "\<And>x. x \<in> set (take (length done) auxlist) \<Longrightarrow> check_before I nt x"
-    using valid_shift_aux by auto
+    using valid_shift_aux unfolding I_def by auto
   have set_drop_auxlist: "\<And>x. x \<in> set (drop (length done) auxlist) \<Longrightarrow> \<not>check_before I nt x"
     using valid_shift_aux[unfolded valid_mmuaux'.simps]
-      list_all2_check_before[OF _ valid_shift_aux(2)] unfolding I_ivl_w by fast
+      list_all2_check_before[OF _ valid_shift_aux(2)] unfolding I_def by fast
   have take_auxlist_takeWhile: "take (length done) auxlist = takeWhile (check_before I nt) auxlist"
     using len_done_auxlist list_all set_drop_auxlist
     by (rule take_length_takeWhile) assumption+
   have rev_done: "rev done = map proj_thd (take (length done) auxlist)"
     using valid_shift_aux by auto
   then have res'_def: "res' = rev done"
-    using eval_until_res[OF assms(4)] unfolding take_auxlist_takeWhile I_ivl_w by auto
+    using eval_until_res[OF assms(4)] unfolding take_auxlist_takeWhile I_def by auto
   then have auxlist'_def: "auxlist' = drop (length done) auxlist"
     using eval_until_auxlist'[OF assms(4)] by auto
-  have eval_mmuaux_eq: "eval_mmuaux nt aux = (rev done, (tp, len, tss, I, pos, maskL, maskR,
+  have eval_mmuaux_eq: "eval_mmuaux args nt aux = (rev done, (tp, tss, len, maskL, maskR,
     a1_map, a2_map, [], 0))"
     using shift_aux_def by auto
   show ?thesis
     using assms(3) done_empty_valid_mmuaux'_intro[OF valid_shift_aux(1)]
-    unfolding shift_aux_def eval_mmuaux_eq b_pos auxlist'_def res'_def valid_mmuaux_def by auto
+    unfolding shift_aux_def eval_mmuaux_eq pos_def auxlist'_def res'_def valid_mmuaux_def by auto
 qed
 
-definition init_mmuaux :: "\<I> \<Rightarrow> bool \<Rightarrow> nat \<Rightarrow> nat set \<Rightarrow> nat set \<Rightarrow> 'a mmuaux" where
-  "init_mmuaux I pos n L R = (0, 0, empty_queue, I, pos, join_mask n L, join_mask n R,
-    Mapping.empty, Mapping.update 0 Mapping.empty Mapping.empty, [], 0)"
+definition init_mmuaux :: "args \<Rightarrow> 'a mmuaux" where
+  "init_mmuaux args = (0, empty_queue, 0,
+  join_mask (args_n args) (args_L args), join_mask (args_n args) (args_R args),
+  Mapping.empty, Mapping.update 0 Mapping.empty Mapping.empty, [], 0)"
 
-lemma valid_init_mmuaux: "L \<subseteq> R \<Longrightarrow> valid_mmuaux (init_window I) pos n L R
-  (init_mmuaux I pos n L R) []"
+lemma valid_init_mmuaux: "L \<subseteq> R \<Longrightarrow> valid_mmuaux (init_args I n L R b) 0
+  (init_mmuaux (init_args I n L R b)) []"
   unfolding init_mmuaux_def valid_mmuaux_def
-  by (auto simp add: init_window_def empty_queue_rep table_def Mapping.lookup_update)
+  by (auto simp add: init_args_def empty_queue_rep table_def Mapping.lookup_update)
 
-fun length_mmuaux :: "'a mmuaux \<Rightarrow> nat" where
-  "length_mmuaux (tp, len, tss, I, pos, maskL, maskR, a1_map, a2_map, done, done_length) =
+fun length_mmuaux :: "args \<Rightarrow> 'a mmuaux \<Rightarrow> nat" where
+  "length_mmuaux args (tp, tss, len, maskL, maskR, a1_map, a2_map, done, done_length) =
     len + done_length"
 
 lemma valid_length_mmuaux:
-  assumes "valid_mmuaux w b n L R aux auxlist"
-  shows "length_mmuaux aux = length auxlist"
+  assumes "valid_mmuaux args cur aux auxlist"
+  shows "length_mmuaux args aux = length auxlist"
   using assms by (cases aux) (auto simp add: valid_mmuaux_def dest: list_all2_lengthD)
 
 end
